<?xml version="1.0"?>
<rdf:RDF xmlns="https://w3id.org/bearchaeo/ArchaeologicalFindingRecord-ontology#"
     xml:base="https://w3id.org/bearchaeo/ArchaeologicalFindingRecord-ontology"
     xmlns:owl="http://www.w3.org/2002/07/owl#"
     xmlns:rdf="http://www.w3.org/1999/02/22-rdf-syntax-ns#"
     xmlns:xml="http://www.w3.org/XML/1998/namespace"
     xmlns:xsd="http://www.w3.org/2001/XMLSchema#"
     xmlns:rdfs="http://www.w3.org/2000/01/rdf-schema#"
     xmlns:skos="http://www.w3.org/2004/02/skos/core#">
    <owl:Ontology rdf:about="https://w3id.org/bearchaeo/ArchaeologicalFindingRecord-ontology#"/>
    


    <!-- 
    ///////////////////////////////////////////////////////////////////////////////////////
    //
    // Annotation properties
    //
    ///////////////////////////////////////////////////////////////////////////////////////
     -->

    


    <!-- http://www.w3.org/2004/02/skos/core#altLabel -->

    <owl:AnnotationProperty rdf:about="http://www.w3.org/2004/02/skos/core#altLabel">
        <rdfs:subPropertyOf rdf:resource="http://www.w3.org/2000/01/rdf-schema#label"/>
    </owl:AnnotationProperty>
    


    <!-- http://www.w3.org/2004/02/skos/core#prefLabel -->

    <owl:AnnotationProperty rdf:about="http://www.w3.org/2004/02/skos/core#prefLabel">
        <rdfs:subPropertyOf rdf:resource="http://www.w3.org/2000/01/rdf-schema#label"/>
    </owl:AnnotationProperty>
    


    <!-- 
    ///////////////////////////////////////////////////////////////////////////////////////
    //
    // Object Properties
    //
    ///////////////////////////////////////////////////////////////////////////////////////
     -->

    


    <!-- https://w3id.org/arco/catalogue/describes -->

    <owl:ObjectProperty rdf:about="https://w3id.org/arco/catalogue/describes"/>
    


    <!-- https://w3id.org/bearchaeo/ArchaeologicalFindingRecord-ontology#describesAF -->

    <owl:ObjectProperty rdf:about="https://w3id.org/bearchaeo/ArchaeologicalFindingRecord-ontology#describesAF">
        <rdfs:subPropertyOf rdf:resource="https://w3id.org/arco/catalogue/describes"/>
        <rdfs:domain rdf:resource="https://w3id.org/bearchaeo/ArchaeologicalFindingRecord-ontology#AF_Record"/>
        <rdfs:range rdf:resource="https://w3id.org/bearchaeo/Archaeo-ontology#ArchaeologicalFinding"/>
        <rdfs:comment>Be Archaeo specialization of the ArCo property &apos;describes&apos;.</rdfs:comment>
        <rdfs:label>describes Archaeological Finding</rdfs:label>
    </owl:ObjectProperty>
    


    <!-- https://w3id.org/bearchaeo/ArchaeologicalFindingRecord-ontology#documentedIn_f -->

    <owl:ObjectProperty rdf:about="https://w3id.org/bearchaeo/ArchaeologicalFindingRecord-ontology#documentedIn_f">
        <rdfs:subPropertyOf rdf:resource="https://w3id.org/bearchaeo/ArchaeologicalFindingRecord-ontology#hasDirectlyRelatedObject_f"/>
        <rdfs:comment>The object property links &apos;directly related object documented in&apos; field to the AF catalogue record.</rdfs:comment>
        <rdfs:label>DIRECTLY RELATED OBJECT
documented in</rdfs:label>
    </owl:ObjectProperty>
    


    <!-- https://w3id.org/bearchaeo/ArchaeologicalFindingRecord-ontology#foundIn_f -->

    <owl:ObjectProperty rdf:about="https://w3id.org/bearchaeo/ArchaeologicalFindingRecord-ontology#foundIn_f">
        <rdfs:subPropertyOf rdf:resource="https://w3id.org/bearchaeo/ArchaeologicalFindingRecord-ontology#hasDirectlyRelatedObject_f"/>
        <rdfs:comment>The object property links &apos;directly related object found in&apos; field to the AF catalogue record.</rdfs:comment>
        <rdfs:label>DIRECTLY RELATED OBJECT
found in</rdfs:label>
    </owl:ObjectProperty>
    


    <!-- https://w3id.org/bearchaeo/ArchaeologicalFindingRecord-ontology#hasComplexObjectRoot_f -->

    <owl:ObjectProperty rdf:about="https://w3id.org/bearchaeo/ArchaeologicalFindingRecord-ontology#hasComplexObjectRoot_f">
        <rdf:type rdf:resource="http://www.w3.org/2002/07/owl#FunctionalProperty"/>
        <rdfs:domain rdf:resource="https://w3id.org/bearchaeo/ArchaeologicalFindingRecord-ontology#AF_Record"/>
        <rdfs:range rdf:resource="https://w3id.org/bearchaeo/ArchaeologicalFindingRecord-ontology#AF_Record"/>
        <rdfs:comment>The object property links &apos;source&apos; field to the AF catalogue record. It encodes the information about the main finding that archaeological finding is a part of.</rdfs:comment>
        <rdfs:label>ROOT of complex object (AF record)</rdfs:label>
    </owl:ObjectProperty>
    


    <!-- https://w3id.org/bearchaeo/ArchaeologicalFindingRecord-ontology#hasDirectlyRelatedObject_f -->

    <owl:ObjectProperty rdf:about="https://w3id.org/bearchaeo/ArchaeologicalFindingRecord-ontology#hasDirectlyRelatedObject_f">
        <rdfs:domain rdf:resource="https://w3id.org/bearchaeo/ArchaeologicalFindingRecord-ontology#AF_Record"/>
        <rdfs:range rdf:resource="https://w3id.org/bearchaeo/ArchaeologicalFindingRecord-ontology#AF_Record"/>
        <rdfs:label>Directly related objects</rdfs:label>
    </owl:ObjectProperty>
    


    <!-- https://w3id.org/bearchaeo/ArchaeologicalFindingRecord-ontology#hasIndirectlyRelatedObject_f -->

    <owl:ObjectProperty rdf:about="https://w3id.org/bearchaeo/ArchaeologicalFindingRecord-ontology#hasIndirectlyRelatedObject_f">
        <rdfs:domain rdf:resource="https://w3id.org/bearchaeo/ArchaeologicalFindingRecord-ontology#AF_Record"/>
        <rdfs:range rdf:resource="https://w3id.org/bearchaeo/ArchaeologicalFindingRecord-ontology#AF_Record"/>
        <rdfs:comment>The object property links &apos;indirectly related object&apos; field to the AF catalogue record.</rdfs:comment>
        <rdfs:label>Indirectly related object (some AF record)</rdfs:label>
    </owl:ObjectProperty>
    


    <!-- https://w3id.org/bearchaeo/ArchaeologicalFindingRecord-ontology#hasSource_f -->

    <owl:ObjectProperty rdf:about="https://w3id.org/bearchaeo/ArchaeologicalFindingRecord-ontology#hasSource_f">
        <rdfs:domain rdf:resource="https://w3id.org/bearchaeo/ArchaeologicalFindingRecord-ontology#AF_Record"/>
        <rdfs:range rdf:resource="https://w3id.org/bearchaeo/suRecord-ontology#SU_catalogueRecord"/>
        <rdfs:comment>The object property links &apos;source&apos; field to the AF catalogue record. It encodes the information about the main resource that finding belongs to. e.g. stratigraphic unit, museum collection or another archaeological finding..</rdfs:comment>
        <rdfs:label>SOURCE</rdfs:label>
    </owl:ObjectProperty>
    


    <!-- https://w3id.org/bearchaeo/ArchaeologicalFindingRecord-ontology#locatedIn_f -->

    <owl:ObjectProperty rdf:about="https://w3id.org/bearchaeo/ArchaeologicalFindingRecord-ontology#locatedIn_f">
        <rdfs:subPropertyOf rdf:resource="https://w3id.org/bearchaeo/ArchaeologicalFindingRecord-ontology#hasDirectlyRelatedObject_f"/>
        <rdfs:comment>The object property links &apos;directly related object located in&apos; field to the AF catalogue record.</rdfs:comment>
        <rdfs:label>DIRECTLY RELATED OBJECT
located in</rdfs:label>
    </owl:ObjectProperty>
    


    <!-- https://w3id.org/bearchaeo/ArchaeologicalFindingRecord-ontology#occurredIn_f -->

    <owl:ObjectProperty rdf:about="https://w3id.org/bearchaeo/ArchaeologicalFindingRecord-ontology#occurredIn_f">
        <rdfs:subPropertyOf rdf:resource="https://w3id.org/bearchaeo/ArchaeologicalFindingRecord-ontology#hasDirectlyRelatedObject_f"/>
        <rdfs:comment>The object property links &apos;directly related object occurred in&apos; field to the AF catalogue record.</rdfs:comment>
        <rdfs:label>DIRECTLY RELATED OBJECT
occurred in</rdfs:label>
    </owl:ObjectProperty>
    


    <!-- https://w3id.org/bearchaeo/ArchaeologicalFindingRecord-ontology#originatedIn_f -->

    <owl:ObjectProperty rdf:about="https://w3id.org/bearchaeo/ArchaeologicalFindingRecord-ontology#originatedIn_f">
        <rdfs:subPropertyOf rdf:resource="https://w3id.org/bearchaeo/ArchaeologicalFindingRecord-ontology#hasDirectlyRelatedObject_f"/>
        <rdfs:comment>The object property links &apos;directly related object originated in&apos; field to the AF catalogue record.</rdfs:comment>
        <rdfs:label>DIRECTLY RELATED OBJECT
originated in</rdfs:label>
    </owl:ObjectProperty>
    


    <!-- https://w3id.org/bearchaeo/ArchaeologicalFindingRecord-ontology#realizedIn_f -->

    <owl:ObjectProperty rdf:about="https://w3id.org/bearchaeo/ArchaeologicalFindingRecord-ontology#realizedIn_f">
        <rdfs:subPropertyOf rdf:resource="https://w3id.org/bearchaeo/ArchaeologicalFindingRecord-ontology#hasDirectlyRelatedObject_f"/>
        <rdfs:comment>The object property links &apos;directly related object realized in&apos; field to the AF catalogue record.</rdfs:comment>
        <rdfs:label>DIRECTLY RELATED OBJECT
realized in</rdfs:label>
    </owl:ObjectProperty>
    


    <!-- https://w3id.org/bearchaeo/ArchaeologicalFindingRecord-ontology#reusedIn_f -->

    <owl:ObjectProperty rdf:about="https://w3id.org/bearchaeo/ArchaeologicalFindingRecord-ontology#reusedIn_f">
        <rdfs:subPropertyOf rdf:resource="https://w3id.org/bearchaeo/ArchaeologicalFindingRecord-ontology#hasDirectlyRelatedObject_f"/>
        <rdfs:comment>The object property links &apos;directly related object reused in&apos; field to the AF catalogue record.</rdfs:comment>
        <rdfs:label>DIRECTLY RELATED OBJECT
reused in</rdfs:label>
    </owl:ObjectProperty>
    


    <!-- https://w3id.org/bearchaeo/ArchaeologicalFindingRecord-ontology#urbanOrEnvironmentalRelatedTo_f -->

    <owl:ObjectProperty rdf:about="https://w3id.org/bearchaeo/ArchaeologicalFindingRecord-ontology#urbanOrEnvironmentalRelatedTo_f">
        <rdfs:subPropertyOf rdf:resource="https://w3id.org/bearchaeo/ArchaeologicalFindingRecord-ontology#hasDirectlyRelatedObject_f"/>
        <rdfs:comment>The object property links &apos;directly related object urban and environmental related to&apos; field to the AF catalogue record.</rdfs:comment>
        <rdfs:label>DIRECTLY RELATED OBJECT
urban or environmental related to</rdfs:label>
    </owl:ObjectProperty>
    


    <!-- 
    ///////////////////////////////////////////////////////////////////////////////////////
    //
    // Data properties
    //
    ///////////////////////////////////////////////////////////////////////////////////////
     -->

    


    <!-- https://w3id.org/bearchaeo/ArchaeologicalFindingRecord-ontology#hasAF_Chronology -->

    <owl:DatatypeProperty rdf:about="https://w3id.org/bearchaeo/ArchaeologicalFindingRecord-ontology#hasAF_Chronology">
        <rdfs:domain rdf:resource="https://w3id.org/bearchaeo/Archaeo-ontology#ArchaeologicalFinding"/>
        <rdfs:range rdf:resource="http://www.w3.org/2001/XMLSchema#string"/>
        <rdfs:comment>This property expresses the data property &apos;AF chronology&apos; field of the archaeological finding record. It encodes one of the fields of the AF catalgoue record.</rdfs:comment>
    </owl:DatatypeProperty>
    


    <!-- https://w3id.org/bearchaeo/ArchaeologicalFindingRecord-ontology#hasAF_ChronologyMotivation_f -->

    <owl:DatatypeProperty rdf:about="https://w3id.org/bearchaeo/ArchaeologicalFindingRecord-ontology#hasAF_ChronologyMotivation_f">
        <rdfs:domain rdf:resource="https://w3id.org/bearchaeo/ArchaeologicalFindingRecord-ontology#AF_Record"/>
        <rdfs:range rdf:resource="http://www.w3.org/2001/XMLSchema#string"/>
        <rdfs:comment>This property expresses the data property &apos;chronology motivation&apos; of the archaeological finding record. It encodes one of the fields of the AF catalogue record.</rdfs:comment>
        <rdfs:label>CHRONOLOGY MOTIVATION</rdfs:label>
    </owl:DatatypeProperty>
    


    <!-- https://w3id.org/bearchaeo/ArchaeologicalFindingRecord-ontology#hasAF_Chronology_f_en -->

    <owl:DatatypeProperty rdf:about="https://w3id.org/bearchaeo/ArchaeologicalFindingRecord-ontology#hasAF_Chronology_f_en">
        <rdfs:subPropertyOf rdf:resource="https://w3id.org/bearchaeo/ArchaeologicalFindingRecord-ontology#hasAF_Chronology"/>
        <rdfs:domain rdf:resource="https://w3id.org/bearchaeo/ArchaeologicalFindingRecord-ontology#AF_Record"/>
        <rdfs:range rdf:resource="http://www.w3.org/2001/XMLSchema#string"/>
        <rdfs:comment>This property expresses the data property &apos;AF number&apos; of the archaeological finding record. It is a subproperty of AF chronology that encodes one of the fields of the AF catalogue record.</rdfs:comment>
        <skos:prefLabel xml:lang="en">CHRONOLOGY</skos:prefLabel>
    </owl:DatatypeProperty>
    


    <!-- https://w3id.org/bearchaeo/ArchaeologicalFindingRecord-ontology#hasAF_Chronology_f_jp -->

    <owl:DatatypeProperty rdf:about="https://w3id.org/bearchaeo/ArchaeologicalFindingRecord-ontology#hasAF_Chronology_f_jp">
        <rdfs:subPropertyOf rdf:resource="https://w3id.org/bearchaeo/ArchaeologicalFindingRecord-ontology#hasAF_Chronology"/>
        <rdfs:domain rdf:resource="https://w3id.org/bearchaeo/ArchaeologicalFindingRecord-ontology#AF_Record"/>
        <rdfs:range rdf:resource="http://www.w3.org/2001/XMLSchema#string"/>
        <rdfs:comment>This property expresses the data property &apos;AF number&apos; of the archaeological finding record. It is a subproperty of AF chronology that encodes one of the fields of the AF catalogue record.</rdfs:comment>
        <skos:prefLabel xml:lang="jp">年表</skos:prefLabel>
    </owl:DatatypeProperty>
    


    <!-- https://w3id.org/bearchaeo/ArchaeologicalFindingRecord-ontology#hasAFnumber_f -->

    <owl:DatatypeProperty rdf:about="https://w3id.org/bearchaeo/ArchaeologicalFindingRecord-ontology#hasAFnumber_f">
        <rdf:type rdf:resource="http://www.w3.org/2002/07/owl#FunctionalProperty"/>
        <rdfs:domain rdf:resource="https://w3id.org/bearchaeo/ArchaeologicalFindingRecord-ontology#AF_Record"/>
        <rdfs:range rdf:resource="http://www.w3.org/2001/XMLSchema#string"/>
        <rdfs:comment>This property expresses the data property &apos;AF number&apos; of the archaeological finding record. It encodes one of the fields of the AF catalogue record.</rdfs:comment>
        <rdfs:label>AF number</rdfs:label>
    </owl:DatatypeProperty>
    


    <!-- https://w3id.org/bearchaeo/ArchaeologicalFindingRecord-ontology#hasBeArchaeoMaterial -->

    <owl:DatatypeProperty rdf:about="https://w3id.org/bearchaeo/ArchaeologicalFindingRecord-ontology#hasBeArchaeoMaterial">
        <rdfs:domain>
            <owl:Class>
                <owl:unionOf rdf:parseType="Collection">
                    <rdf:Description rdf:about="https://w3id.org/bearchaeo/Archaeo-ontology#ArchaeologicalFinding"/>
                    <rdf:Description rdf:about="https://w3id.org/bearchaeo/ArchaeologicalFindingRecord-ontology#AF_Record"/>
                </owl:unionOf>
            </owl:Class>
        </rdfs:domain>
        <rdfs:range rdf:resource="http://www.w3.org/2001/XMLSchema#string"/>
        <rdfs:comment>This property expresses the data property &apos;object definition according to Be-Archaeo thesaurus&apos; of the archaeological finding record. It encodes one of the fields of the AF catalogue record.</rdfs:comment>
        <rdfs:label>Object definition (Be-Archaeo thesaurus)</rdfs:label>
    </owl:DatatypeProperty>
    


    <!-- https://w3id.org/bearchaeo/ArchaeologicalFindingRecord-ontology#hasComplexObjectLevel_f -->

    <owl:DatatypeProperty rdf:about="https://w3id.org/bearchaeo/ArchaeologicalFindingRecord-ontology#hasComplexObjectLevel_f">
        <rdf:type rdf:resource="http://www.w3.org/2002/07/owl#FunctionalProperty"/>
        <rdfs:domain rdf:resource="https://w3id.org/bearchaeo/ArchaeologicalFindingRecord-ontology#AF_Record"/>
        <rdfs:range rdf:resource="http://www.w3.org/2001/XMLSchema#string"/>
        <rdfs:comment>This property expresses the data property &apos;level for complex objects&apos; of the archaeological finding record. It encodes one of the fields of the AF catalogue record.</rdfs:comment>
        <rdfs:label>Level (X.Y. ... .Z) - for complex objects</rdfs:label>
    </owl:DatatypeProperty>
    


    <!-- https://w3id.org/bearchaeo/ArchaeologicalFindingRecord-ontology#hasGettyAAT_Material -->

    <owl:DatatypeProperty rdf:about="https://w3id.org/bearchaeo/ArchaeologicalFindingRecord-ontology#hasGettyAAT_Material">
        <rdfs:domain>
            <owl:Class>
                <owl:unionOf rdf:parseType="Collection">
                    <rdf:Description rdf:about="https://w3id.org/bearchaeo/Archaeo-ontology#ArchaeologicalFinding"/>
                    <rdf:Description rdf:about="https://w3id.org/bearchaeo/ArchaeologicalFindingRecord-ontology#AF_Record"/>
                </owl:unionOf>
            </owl:Class>
        </rdfs:domain>
        <rdfs:range rdf:resource="http://www.w3.org/2001/XMLSchema#string"/>
        <rdfs:comment>This property expresses the data property &apos;object definition according to Getty-AAT thesaurus&apos; of the archaeological finding record. It encodes one of the fields of the AF catalogue record.</rdfs:comment>
        <rdfs:label>Object definition (Getty-AAT thesaurus)</rdfs:label>
    </owl:DatatypeProperty>
    


    <!-- 
    ///////////////////////////////////////////////////////////////////////////////////////
    //
    // Classes
    //
    ///////////////////////////////////////////////////////////////////////////////////////
     -->

    


    <!-- https://w3id.org/bearchaeo/Archaeo-ontology#ArchaeologicalFinding -->

    <owl:Class rdf:about="https://w3id.org/bearchaeo/Archaeo-ontology#ArchaeologicalFinding"/>
    


    <!-- https://w3id.org/bearchaeo/ArchaeologicalFindingRecord-ontology#AF_Record -->

    <owl:Class rdf:about="https://w3id.org/bearchaeo/ArchaeologicalFindingRecord-ontology#AF_Record">
        <rdfs:comment>Archaeological finding&apos;s catalogue record that describes the information about the finding.</rdfs:comment>
        <rdfs:label>Archaeological finding record</rdfs:label>
    </owl:Class>
    


    <!-- https://w3id.org/bearchaeo/suRecord-ontology#SU_catalogueRecord -->

    <owl:Class rdf:about="https://w3id.org/bearchaeo/suRecord-ontology#SU_catalogueRecord">
        <rdfs:comment>Stratigraphic unit&apos;s catalogue record that describes the information about the unit.</rdfs:comment>
    </owl:Class>
</rdf:RDF>



<!-- Generated by the OWL API (version 4.5.9.2019-02-01T07:24:44Z) https://github.com/owlcs/owlapi -->

