@prefix : <https://saref.etsi.org/saref4auto/> .
@prefix dc: <http://purl.org/dc/elements/1.1/> .
@prefix sf: <http://www.opengis.net/ont/sf#> .
@prefix owl: <http://www.w3.org/2002/07/owl#> .
@prefix rdf: <http://www.w3.org/1999/02/22-rdf-syntax-ns#> .
@prefix xml: <http://www.w3.org/XML/1998/namespace> .
@prefix xsd: <http://www.w3.org/2001/XMLSchema#> .
@prefix rdfs: <http://www.w3.org/2000/01/rdf-schema#> .
@prefix time: <http://www.w3.org/2006/time#> .
@prefix vann: <http://purl.org/vocab/vann/> .
@prefix geosp: <http://www.opengis.net/ont/geosparql#> .
@prefix saref: <https://saref.etsi.org/core/> .
@prefix s4auto: <https://saref.etsi.org/saref4auto/> .
@prefix s4city: <https://saref.etsi.org/saref4city/> .
@prefix s4syst: <https://saref.etsi.org/saref4syst/> .
@prefix dcterms: <http://purl.org/dc/terms/> .
@base <https://saref.etsi.org/saref4auto/> .

<https://saref.etsi.org/saref4auto/> rdf:type owl:Ontology ;
                                      owl:versionIRI <https://saref.etsi.org/saref4auto/v1.1.1/> ;
                                      dcterms:contributor <https://scholar.google.com/citations?user=coCDIj8AAAAJ> ;
                                      dcterms:creator <http://netellany.fr/> ,
                                                      <https://www.linkedin.com/in/lauradaniele> ;
                                      dcterms:description "This ontology extends the SAREF ontology for the automotive domain. This work has been developed in the context of the STF 566, which was established with the goal to create four SAREF extensions, one of them for the automotive domain."@en ;
                                      dcterms:issued "2020-07-27"^^xsd:date ;
                                      dcterms:license <https://forge.etsi.org/etsi-software-license> ;
                                      dcterms:modified "2021-07-26"^^xsd:date ;
                                      dcterms:publisher <https://www.etsi.org/> ;
                                      dcterms:source <https://saref.etsi.org/sources/saref4auto/> ;
                                      dcterms:title "SAREF extension for automotive"@en ;
                                      vann:preferredNamespacePrefix "s4auto" ;
                                      vann:preferredNamespaceUri "https://saref.etsi.org/saref4auto/" ;
                                      rdfs:seeAlso <https://www.etsi.org/deliver/etsi_ts/103400_103499/10341007/01.01.01_60/ts_10341007v010101p.pdf> ;
                                      owl:versionInfo "v1.1.1" .

#################################################################
#    Annotation properties
#################################################################

###  http://purl.org/dc/terms/contributor
dcterms:contributor rdf:type owl:AnnotationProperty .


###  http://purl.org/dc/terms/creator
dcterms:creator rdf:type owl:AnnotationProperty .


###  http://purl.org/dc/terms/description
dcterms:description rdf:type owl:AnnotationProperty .


###  http://purl.org/dc/terms/issued
dcterms:issued rdf:type owl:AnnotationProperty .


###  http://purl.org/dc/terms/license
dcterms:license rdf:type owl:AnnotationProperty .


###  http://purl.org/dc/terms/modified
dcterms:modified rdf:type owl:AnnotationProperty .


###  http://purl.org/dc/terms/publisher
dcterms:publisher rdf:type owl:AnnotationProperty .


###  http://purl.org/dc/terms/source
dcterms:source rdf:type owl:AnnotationProperty .


###  http://purl.org/dc/terms/title
dcterms:title rdf:type owl:AnnotationProperty .


###  http://purl.org/vocab/vann/preferredNamespacePrefix
vann:preferredNamespacePrefix rdf:type owl:AnnotationProperty .


###  http://purl.org/vocab/vann/preferredNamespaceUri
vann:preferredNamespaceUri rdf:type owl:AnnotationProperty .


#################################################################
#    Object Properties
#################################################################

###  http://www.opengis.net/ont/geosparql#hasGeometry
geosp:hasGeometry rdf:type owl:ObjectProperty ;
                  rdfs:domain geosp:Feature ;
                  rdfs:range geosp:Geometry ;
                  rdfs:comment "A spatial representation for a given feature." ;
                  rdfs:isDefinedBy <http://www.opengis.net/ont/geosparql> .


###  http://www.w3.org/2003/01/geo/wgs84_pos#location
<http://www.w3.org/2003/01/geo/wgs84_pos#location> rdf:type owl:ObjectProperty ;
                                                   rdfs:range <http://www.w3.org/2003/01/geo/wgs84_pos#SpatialThing> ;
                                                   rdfs:comment """The relation between something and the point, 
 or other geometrical thing in space, where it is.  For example, the realtionship between
 a radio tower and a Point with a given lat and long.
 Or a relationship between a park and its outline as a closed arc of points, or a road and
 its location as a arc (a sequence of points).
 Clearly in practice there will be limit to the accuracy of any such statement, but one would expect
 an accuracy appropriate for the size of the object and uses such as mapping .""" ;
                                                   rdfs:isDefinedBy "http://www.w3.org/2003/01/geo/wgs84_pos#" ;
                                                   rdfs:label "location"@en .


###  http://www.w3.org/2006/time#hasBeginning
time:hasBeginning rdf:type owl:ObjectProperty ;
                  rdfs:domain time:TemporalEntity ;
                  rdfs:range time:Instant ;
                  rdfs:comment "Beginning of a temporal entity" ;
                  rdfs:isDefinedBy "http://www.w3.org/2006/time" ;
                  rdfs:label "hasBeginning"@en .


###  http://www.w3.org/2006/time#hasEnd
time:hasEnd rdf:type owl:ObjectProperty ;
            rdfs:domain time:TemporalEntity ;
            rdfs:range time:Instant ;
            rdfs:comment "End of a temporal entity." ;
            rdfs:isDefinedBy "http://www.w3.org/2006/time" ;
            rdfs:label "hasEnd"@en .


###  https://saref.etsi.org/core/consistsOf
saref:consistsOf rdf:type owl:ObjectProperty ;
                 rdfs:comment "A relationship indicating a composite entity that consists of other entities (e.g., a temperature/humidity sensor that consists of a temperature sensor and a humidity sensor)"@en ;
                 rdfs:isDefinedBy <https://saref.etsi.org/core> ;
                 rdfs:label "consists of"@en .


###  https://saref.etsi.org/core/controlsProperty
saref:controlsProperty rdf:type owl:ObjectProperty ;
                       rdfs:comment "A relationship specifying the property that can be controlled by a certain device"@en ;
                       rdfs:isDefinedBy saref: ;
                       rdfs:label "controls property"@en .


###  https://saref.etsi.org/core/hasProperty
saref:hasProperty rdf:type owl:ObjectProperty ;
                  rdfs:domain saref:FeatureOfInterest ;
                  rdfs:range saref:Property ;
                  rdfs:comment "A relationship between a feature of interest and a property of that feature"@en ;
                  rdfs:isDefinedBy saref: ;
                  rdfs:label "controls property"@en .


###  https://saref.etsi.org/core/isControlledByDevice
saref:isControlledByDevice rdf:type owl:ObjectProperty ;
                           rdfs:comment "A relationship specifying the devices that can control a certain property"@en ;
                           rdfs:isDefinedBy saref: ;
                           rdfs:label "is controlled by device"@en .


###  https://saref.etsi.org/core/isMeasuredByDevice
saref:isMeasuredByDevice rdf:type owl:ObjectProperty ;
                         rdfs:domain saref:Measurement ;
                         rdfs:comment "A relationship specifying the devices that can measure a certain property"@en ;
                         rdfs:isDefinedBy saref: ;
                         rdfs:label "is measured by device"@en .


###  https://saref.etsi.org/core/isMeasuredIn
saref:isMeasuredIn rdf:type owl:ObjectProperty ;
                   rdfs:comment "A relationship identifying the unit of measure used for a certain entity."@en ;
                   rdfs:isDefinedBy saref: ;
                   rdfs:label "is measured in"@en .


###  https://saref.etsi.org/core/makesMeasurement
saref:makesMeasurement rdf:type owl:ObjectProperty ;
                       owl:inverseOf saref:measurementMadeBy ;
                       rdfs:comment "A relation between a device and the measurements it makes. Such measurement will link together the value of the measurement, its unit of measure and the property to which it relates."@en ;
                       rdfs:isDefinedBy saref: ;
                       rdfs:label "makes measurement"@en .


###  https://saref.etsi.org/core/measurementMadeBy
saref:measurementMadeBy rdf:type owl:ObjectProperty ;
                        rdfs:comment "A relation between a measurement and the device that made it."@en ;
                        rdfs:isDefinedBy saref: ;
                        rdfs:label "measurementMadeBy"@en .


###  https://saref.etsi.org/core/measuresProperty
saref:measuresProperty rdf:type owl:ObjectProperty ;
                       rdfs:domain saref:Device ;
                       rdfs:range saref:Property ;
                       rdfs:comment "A relationship specifying the property that can be measured by a certain device"@en ;
                       rdfs:isDefinedBy saref: ;
                       rdfs:label "measures property"@en .


###  https://saref.etsi.org/core/relatesToMeasurement
saref:relatesToMeasurement rdf:type owl:ObjectProperty ;
                           rdfs:comment "A relationship between a property and the measurements it relates to"@en ;
                           rdfs:isDefinedBy saref: ;
                           rdfs:label "relates to measurement"@en .


###  https://saref.etsi.org/core/relatesToProperty
saref:relatesToProperty rdf:type owl:ObjectProperty ;
                        rdfs:comment "A relationship between a measurement and the property it relates to"@en ;
                        rdfs:isDefinedBy saref: ;
                        rdfs:label "relates to property"@en .


###  https://saref.etsi.org/saref4auto/OWLObjectProperty_10d4f71b_6da1_4eb5_840c_760db83f999d
s4auto:OWLObjectProperty_10d4f71b_6da1_4eb5_840c_760db83f999d rdf:type owl:ObjectProperty ;
                                                              rdfs:comment "File format to storage the data" ;
                                                              rdfs:label "hasFormat"@es .


###  https://saref.etsi.org/saref4auto/OWLObjectProperty_1828ea5b_6175_4e01_88e4_a1b9cab3b318
s4auto:OWLObjectProperty_1828ea5b_6175_4e01_88e4_a1b9cab3b318 rdf:type owl:ObjectProperty ;
                                                              rdfs:comment "Exists a relation between classes" ;
                                                              rdfs:label "is related to"@es .


###  https://saref.etsi.org/saref4auto/OWLObjectProperty_c016f3d4_1a3a_4a8b_b22d_56aaff72f689
s4auto:OWLObjectProperty_c016f3d4_1a3a_4a8b_b22d_56aaff72f689 rdf:type owl:ObjectProperty ;
                                                              rdfs:label "hasProperty"@es .


###  https://saref.etsi.org/saref4auto/OWLObjectProperty_e1bbccf3_d604_4a6c_a130_e2148e0787fc
s4auto:OWLObjectProperty_e1bbccf3_d604_4a6c_a130_e2148e0787fc rdf:type owl:ObjectProperty ;
                                                              rdfs:domain s4auto:OWLClass_f2f0f1ca_8879_4599_8acf_34fcb5e0c2a6 ;
                                                              rdfs:range s4auto:OWLClass_553f9409_f262_4ed9_a940_180eb68bbb2a ;
                                                              rdfs:label "hasDataOf"@es .


###  https://saref.etsi.org/saref4auto/consistsOfEntity
s4auto:consistsOfEntity rdf:type owl:ObjectProperty ;
                        rdfs:subPropertyOf saref:consistsOf ;
                        rdfs:comment "A relation to describe the entities that can compose the vehicle environment"@en ;
                        rdfs:label "consists Of Entity"@en .


###  https://saref.etsi.org/saref4auto/consistsOfEquipment
s4auto:consistsOfEquipment rdf:type owl:ObjectProperty ;
                           rdfs:subPropertyOf saref:consistsOf ;
                           rdfs:comment "A relation to describe the type of equipment that can compose the vehicle environment"@en ;
                           rdfs:label "consists of equipment"@en .


###  https://saref.etsi.org/saref4auto/consistsOfEvent
s4auto:consistsOfEvent rdf:type owl:ObjectProperty ;
                       rdfs:subPropertyOf saref:consistsOf ;
                       rdfs:comment "A relation to describe the events that can compose the vehicle environment"@en ;
                       rdfs:label "consists of event"@en .


###  https://saref.etsi.org/saref4auto/consistsOfObject
s4auto:consistsOfObject rdf:type owl:ObjectProperty ;
                        rdfs:subPropertyOf saref:consistsOf ;
                        rdfs:comment "A relation to describe the objects that can compose the vehicle environment"@en ;
                        rdfs:label "consists of object"@en .


###  https://saref.etsi.org/saref4auto/consistsOfUser
s4auto:consistsOfUser rdf:type owl:ObjectProperty ;
                      rdfs:subPropertyOf saref:consistsOf ;
                      rdfs:comment "A relation to describe the users that can compose the vehicle environment"@en ;
                      rdfs:label "consists of user"@en .


###  https://saref.etsi.org/saref4auto/consistsOfVehicle
s4auto:consistsOfVehicle rdf:type owl:ObjectProperty ;
                         rdfs:subPropertyOf saref:consistsOf ;
                         rdfs:comment "A relation to decribe the vehicles that can compose the vehicle environment"@en ;
                         rdfs:label "consists of vehicle"@en .


###  https://saref.etsi.org/saref4auto/detectsPosition
s4auto:detectsPosition rdf:type owl:ObjectProperty ;
                       rdfs:comment "A relationship specifying the position (absolute or relative position) that can be detected by a certain device"@en ;
                       rdfs:label "detects position"@en .


###  https://saref.etsi.org/saref4auto/hasAbsolutePosition
s4auto:hasAbsolutePosition rdf:type owl:ObjectProperty ;
                           rdfs:subPropertyOf s4auto:hasPosition ;
                           rdfs:comment "A relation between an entity, e.g., a vehicle or road entity, and AbsolutePosition to represent its absolute position"@en ;
                           rdfs:label "hasAbsolutePosition"@en .


###  https://saref.etsi.org/saref4auto/hasAutomationLevel
s4auto:hasAutomationLevel rdf:type owl:ObjectProperty ;
                          rdfs:comment """A relation to define the level of automation of a singular vehicle. According to SAE J3016, there are five levels of automation:
- Level 0: No Driving Automation.
- Level 1: Driver assistance.
- Level 2: Partial driving automation.
- Level 3: Conditional driving automation.
- Level 4: High driving automation.
- Level 5: Full Driving automation.
."""@en ;
                          rdfs:label "hasAutomationLevel"@en .


###  https://saref.etsi.org/saref4auto/hasBrakeCapacity
s4auto:hasBrakeCapacity rdf:type owl:ObjectProperty ;
                        rdfs:range s4auto:BrakeCapacity ;
                        rdfs:comment "A relation to express that the vehicle has the capacity to reduce its speed (by action on the brake pedal or an autonomous actuator)"@en ;
                        rdfs:label "hasBrakeCapacity"@en .


###  https://saref.etsi.org/saref4auto/hasConfidence
s4auto:hasConfidence rdf:type owl:ObjectProperty ;
                     owl:inverseOf s4auto:isConfidenceOf ;
                     rdfs:range s4auto:Confidence ;
                     rdfs:comment "A relation between an estimated measurement (saref:Measurement class) and its confidence (s4auto:Confidence)"@en ;
                     rdfs:label "hasConfidence"@en .


###  https://saref.etsi.org/saref4auto/hasConfidenceUnitOfMeasure
s4auto:hasConfidenceUnitOfMeasure rdf:type owl:ObjectProperty ;
                                  rdfs:comment "A relation that allows to specify the unit of measure associated with a certain confidence"@en ;
                                  rdfs:label "has confidence unit of measure"@en .


###  https://saref.etsi.org/saref4auto/hasDestination
s4auto:hasDestination rdf:type owl:ObjectProperty ;
                      rdfs:comment "A relation that defines the destination of an automotive object. For example, in a platoon, the current platoon leader defines the platoon destination. Following vehicles will share (partially) the route of the leader and can, therefore, have different final destinations." ;
                      rdfs:label "hasDestination"@en .


###  https://saref.etsi.org/saref4auto/hasDestinationAddress
s4auto:hasDestinationAddress rdf:type owl:ObjectProperty ;
                             rdfs:subPropertyOf s4auto:hasDestination ;
                             rdfs:comment "A relation to express the destination of a vehicle in terms of an Address"@en ;
                             rdfs:label "hasDestinationAddress"@en .


###  https://saref.etsi.org/saref4auto/hasDestinationEndPoint
s4auto:hasDestinationEndPoint rdf:type owl:ObjectProperty ;
                              rdfs:subPropertyOf s4auto:hasDestination ;
                              rdfs:comment "A relation to express the destination of a vehicle, a platoon or a route in terms of an end point with latitude and longitude"@en ;
                              rdfs:label "hasDestinationEndPoint"@en .


###  https://saref.etsi.org/saref4auto/hasEnvironment
s4auto:hasEnvironment rdf:type owl:ObjectProperty ;
                      rdfs:comment "A relation that allows to describe the environment of a vehicle"@en ;
                      rdfs:label "hasEnvironment"@en .


###  https://saref.etsi.org/saref4auto/hasEstimatedRendezvousLocation
s4auto:hasEstimatedRendezvousLocation rdf:type owl:ObjectProperty ;
                                      rdfs:range s4auto:RendezvousLocation ;
                                      rdfs:comment "A relation to express that, during the forming state, a vehicle member of a platoon is given an estimated rendezvous location for joining the platoon. It is expressed in global coordinates (lat, long, alt), e.g. according to WGS 84." ;
                                      rdfs:label "hasEstimatedRendezvousLocation"@en .


###  https://saref.etsi.org/saref4auto/hasHeight
s4auto:hasHeight rdf:type owl:ObjectProperty ;
                 rdfs:subPropertyOf saref:hasProperty ;
                 rdfs:comment "A relation to express the height of an entity, e.g., a vehicle or an entity in the vehicle environment"@en ;
                 rdfs:label "hasHeight"@en .


###  https://saref.etsi.org/saref4auto/hasIdentifier
s4auto:hasIdentifier rdf:type owl:ObjectProperty ;
                     rdfs:range s4auto:Identifier ;
                     rdfs:comment "A relation between an entity and its identifier (s4auto:Identifier) which is used to identify 1) a vehicle (station) during data exchange with other devices/stations 2) a platoon during data exchange with other devices/stations, 3) a parking spot within a parking area during data exchange with other devices/stations. In all cases, this identifier may be a pseudonym. It may change over space and/or over time."@en ;
                     rdfs:label "hasIdentifier"@en .


###  https://saref.etsi.org/saref4auto/hasLength
s4auto:hasLength rdf:type owl:ObjectProperty ;
                 rdfs:subPropertyOf saref:hasProperty ;
                 rdfs:comment "A relation to express the length of an entity, e.g., a vehicle or an entity in the vehicle environment or a platoon (Length of the platoon is the sum of all vehicles' length + inter-vehicle distance)"@en ;
                 rdfs:label "hasLength"@en .


###  https://saref.etsi.org/saref4auto/hasMember
s4auto:hasMember rdf:type owl:ObjectProperty ;
                 owl:inverseOf s4auto:isMemberOf ;
                 rdfs:comment "A general relationship to express that an entity can have members"@en ;
                 rdfs:label "hasMember"@en .


###  https://saref.etsi.org/saref4auto/hasMovement
s4auto:hasMovement rdf:type owl:ObjectProperty ;
                   rdfs:subPropertyOf saref:hasProperty ;
                   rdfs:comment "A relation to express the movement of an entity in the vehicle environment."@en ;
                   rdfs:label "hasMovement"@en .


###  https://saref.etsi.org/saref4auto/hasOpeningTimeAvailability
s4auto:hasOpeningTimeAvailability rdf:type owl:ObjectProperty ;
                                  rdfs:comment "A relation to express the opening time of parking spot"@en ;
                                  rdfs:label "hasOpeningTimeAvailability"@en .


###  https://saref.etsi.org/saref4auto/hasOrigin
s4auto:hasOrigin rdf:type owl:ObjectProperty ;
                 rdfs:comment "A relation to express the origin of an entity (e.g., a vehicle or a route)  in terms of a StartPoint"@en ;
                 rdfs:label "hasOrigin"@en .


###  https://saref.etsi.org/saref4auto/hasParkingSpotState
s4auto:hasParkingSpotState rdf:type owl:ObjectProperty ;
                           rdfs:subPropertyOf s4auto:hasState ;
                           rdfs:comment "A relation to express the state of a parking spot"@en ;
                           rdfs:label "hasParkingSpotState"@en .


###  https://saref.etsi.org/saref4auto/hasParkingVehicleState
s4auto:hasParkingVehicleState rdf:type owl:ObjectProperty ;
                              rdfs:subPropertyOf s4auto:hasState ;
                              rdfs:comment "A relation to express the state of a vehicle that is parking"@en ;
                              rdfs:label "hasParkingVehicleState"@en .


###  https://saref.etsi.org/saref4auto/hasPerceptionState
s4auto:hasPerceptionState rdf:type owl:ObjectProperty ;
                          rdfs:subPropertyOf s4auto:hasState ;
                          rdfs:comment "A relation to express the state of a vehicle related to its environment"@en ;
                          rdfs:label "hasPerceptionState"@en .


###  https://saref.etsi.org/saref4auto/hasPlatoonMember
s4auto:hasPlatoonMember rdf:type owl:ObjectProperty ;
                        rdfs:subPropertyOf s4auto:hasMember ;
                        rdfs:comment "A relation to express that a platoon can have vehicles as its members"@en ;
                        rdfs:label "hasPlatoonMember"@en .


###  https://saref.etsi.org/saref4auto/hasPlatoonPosition
s4auto:hasPlatoonPosition rdf:type owl:ObjectProperty ;
                          rdfs:subPropertyOf s4auto:hasPosition ;
                          rdfs:comment "A relatiA relation to express that a vehicle member of a platoon has a platoon position that is defined as the index of the vehicle in the platoon starting from zero (leader) up to N (trailing vehicle)"@en ;
                          rdfs:label "hasPlatoonPosition"@en .


###  https://saref.etsi.org/saref4auto/hasPlatoonRole
s4auto:hasPlatoonRole rdf:type owl:ObjectProperty ;
                      rdfs:subPropertyOf s4auto:hasRole ;
                      rdfs:comment "A relation to specify that in a platoon a vehicle can assume roles such as: unknown, leader, follower, ready-for-leading, trailing, etc."@en ;
                      rdfs:label "hasPlatoonRole"@en .


###  https://saref.etsi.org/saref4auto/hasPlatoonState
s4auto:hasPlatoonState rdf:type owl:ObjectProperty ;
                       rdfs:subPropertyOf s4auto:hasState ;
                       rdfs:comment "A relation to express the state of a platoon"@en ;
                       rdfs:label "hasPlatoonState"@en .


###  https://saref.etsi.org/saref4auto/hasPlatoonVehicleState
s4auto:hasPlatoonVehicleState rdf:type owl:ObjectProperty ;
                              rdfs:subPropertyOf s4auto:hasState ;
                              rdfs:comment "A relation to express the state of a vehicle in a platoon"@en ;
                              rdfs:label "hasPlatoonVehicleState"@en .


###  https://saref.etsi.org/saref4auto/hasPosition
s4auto:hasPosition rdf:type owl:ObjectProperty ;
                   rdfs:range s4auto:RelativePosition ;
                   rdfs:comment "A relation to define the position of an entity"@en ;
                   rdfs:label "has position"@en .


###  https://saref.etsi.org/saref4auto/hasRelativePosition
s4auto:hasRelativePosition rdf:type owl:ObjectProperty ;
                           rdfs:subPropertyOf s4auto:hasPosition ;
                           rdfs:comment "A relation between an entity, e.g., a vehicle or road entity, and RelativePosition to represent its relative position (e.g., a car is x,y,z in front of another car)"@en ;
                           rdfs:label "hasPlatoonPosition"@en .


###  https://saref.etsi.org/saref4auto/hasRoadTopologyPosition
s4auto:hasRoadTopologyPosition rdf:type owl:ObjectProperty ;
                               rdfs:subPropertyOf s4auto:hasPosition ;
                               rdfs:comment "A relation between Vehicle and RoadTopologyPosition to represent the road topology position of a vehicle"@en ;
                               rdfs:label "hasRoadTopologyPosition"@en .


###  https://saref.etsi.org/saref4auto/hasRole
s4auto:hasRole rdf:type owl:ObjectProperty ;
               rdfs:range s4auto:Role ;
               rdfs:comment "A general relation to express that an entity can have a role"@en ;
               rdfs:label "hasRole"@en .


###  https://saref.etsi.org/saref4auto/hasRoute
s4auto:hasRoute rdf:type owl:ObjectProperty ;
                rdfs:comment "A relation to express the route of an entity, e.g., a vehicle or a platoon"@en ;
                rdfs:label "hasRoute"@en .


###  https://saref.etsi.org/saref4auto/hasShape
s4auto:hasShape rdf:type owl:ObjectProperty ;
                rdfs:subPropertyOf saref:hasProperty ;
                rdfs:comment "A relation to express the shape of an entity in the vehicle environment."@en ;
                rdfs:label "hasShape"@en .


###  https://saref.etsi.org/saref4auto/hasSize
s4auto:hasSize rdf:type owl:ObjectProperty ;
               rdfs:subPropertyOf saref:hasProperty ;
               rdfs:comment "A relation to express that a platoon has a size. This size is defined as 1) the total number of vehicles currently in the platoon; or 2) Length of the platoon (sum of all vehicles' length + inter-vehicle distance) via s4auto:hasLength property"@en ;
               rdfs:label "hasSize"@en .


###  https://saref.etsi.org/saref4auto/hasState
s4auto:hasState rdf:type owl:ObjectProperty ;
                rdfs:comment "An hasState relation to connect to a certain state. The saref:hasState property could not be reused because it has domain saref:Device, but a s4auto:Platoon or s4auto:Vehicle are not devices. Therefore, a new s4auto:hasState property with subroperties has been created."@en ;
                rdfs:label "hasState"@en .


###  https://saref.etsi.org/saref4auto/hasVehicleEnvironmentMember
s4auto:hasVehicleEnvironmentMember rdf:type owl:ObjectProperty ;
                                   rdfs:subPropertyOf s4auto:hasMember ;
                                   rdfs:comment "A relation to express that a vehicle can have members in its environment"@en ;
                                   rdfs:label "hasVehicleEnvironmentMember"@en .


###  https://saref.etsi.org/saref4auto/hasVehicleRole
s4auto:hasVehicleRole rdf:type owl:ObjectProperty ;
                      rdfs:subPropertyOf s4auto:hasRole ;
                      rdfs:comment "A relation between Vehicle and VehicleRole classes, to express the role the vehicle plays in traffic. If not specified, it is assumed that it takes a default value. Otherwise, possible values to be specified are: publicTransport, specialTransport, dangerousGoods, roadWork, rescue, emergency, safetyCar, agriculture, commercial, military, roadOperator, taxi (see ETSI TR 103 508)."@en ;
                      rdfs:label "hasVehicleRole"@en .


###  https://saref.etsi.org/saref4auto/hasWidth
s4auto:hasWidth rdf:type owl:ObjectProperty ;
                rdfs:subPropertyOf saref:hasProperty ;
                rdfs:comment "A relation to express the width of an entity, e.g., a vehicle or an entity in the vehicle environment"@en ;
                rdfs:label "hasWidth"@en .


###  https://saref.etsi.org/saref4auto/isCollectionOf
s4auto:isCollectionOf rdf:type owl:ObjectProperty ;
                      rdfs:comment "A relation to express the intermediate destination of a route (e.g., of a vehicle or a platoon) in terms of RoutePoint"@en ;
                      rdfs:label "isCollectionOf"@en .


###  https://saref.etsi.org/saref4auto/isConfidenceOf
s4auto:isConfidenceOf rdf:type owl:ObjectProperty ;
                      rdfs:comment "A relation between the confidence (s4auto:Confidence class) of an estimated measurement and this measurement (saref:Measurement class)"@en ;
                      rdfs:label "isConfidenceOf"@en .


###  https://saref.etsi.org/saref4auto/isMemberOf
s4auto:isMemberOf rdf:type owl:ObjectProperty ;
                  rdfs:comment "A general relationship to express that an entity is a member of another entity"@en ;
                  rdfs:label "isMemberOf"@en .


###  https://saref.etsi.org/saref4auto/isMemberOfPlatoon
s4auto:isMemberOfPlatoon rdf:type owl:ObjectProperty ;
                         rdfs:subPropertyOf s4auto:isMemberOf ;
                         rdfs:comment "A relation to express that a vehicle can be member of  a platoon"@en ;
                         rdfs:label "isMemberOfPlatoon"@en .


###  https://saref.etsi.org/saref4auto/isMemberOfVehicleEnvironment
s4auto:isMemberOfVehicleEnvironment rdf:type owl:ObjectProperty ;
                                    rdfs:subPropertyOf s4auto:isMemberOf ;
                                    rdfs:comment "A relation to express that an entity, e.g., a vehicle, can be member of  another vehicle's environment"@en ;
                                    rdfs:label "isMemberOfVehicleEnvironment"@en .


###  https://saref.etsi.org/saref4auto/usesMeasurement
s4auto:usesMeasurement rdf:type owl:ObjectProperty ;
                       rdfs:comment "A relation to express that a device can use different types of measurements, such as speed, position of detected road objects (e.g., bicycles, vehicles). This applies in particular to the ElectronicControlUnit and TrafficLightController classes."@en ;
                       rdfs:label "usesMeasurement"@en .


###  https://saref.etsi.org/saref4syst/hasSubSystem
s4syst:hasSubSystem rdf:type owl:ObjectProperty ;
                    owl:inverseOf s4syst:subSystemOf ;
                    rdfs:comment "In SAREF4AUTO, a  relation to express that the vehicle has a subsystem called ‘ElectronicControlUnit' (ECU) that provides measurements about relevant properties, such as speed, acceleration, position, etc."@en ,
                                 "Links a system to one of its sub systems"@en ;
                    rdfs:isDefinedBy s4syst: ;
                    rdfs:label "hasSubSystem"@en .


###  https://saref.etsi.org/saref4syst/subSystemOf
s4syst:subSystemOf rdf:type owl:ObjectProperty ;
                   rdfs:comment "In SAREF4AUTO, a relation to express that the the ElectronicControlUnit (ECU) is a subsystem of the vehicle."@en ,
                                "Links a system to its super system. Properties of subsystems somehow contribute to the properties of the super system. The exact meaning of \"contribute is defined by sub properties of s4syst:subSystemOf. Property s4syst:subSystemOf is transitive."@en ;
                   rdfs:isDefinedBy s4syst: ;
                   rdfs:label "subSystemOf"@en .


#################################################################
#    Data properties
#################################################################

###  http://www.w3.org/2003/01/geo/wgs84_pos#alt
<http://www.w3.org/2003/01/geo/wgs84_pos#alt> rdf:type owl:DatatypeProperty ;
                                              rdfs:domain <http://www.w3.org/2003/01/geo/wgs84_pos#SpatialThing> ;
                                              rdfs:comment """The WGS84 altitude of a SpatialThing (decimal meters 
above the local reference ellipsoid).""" ;
                                              rdfs:isDefinedBy "http://www.w3.org/2003/01/geo/wgs84_pos" ;
                                              rdfs:label "altitude" .


###  http://www.w3.org/2003/01/geo/wgs84_pos#lat
<http://www.w3.org/2003/01/geo/wgs84_pos#lat> rdf:type owl:DatatypeProperty ;
                                              rdfs:domain <http://www.w3.org/2003/01/geo/wgs84_pos#SpatialThing> ;
                                              rdfs:comment "The WGS84 latitude of a SpatialThing (decimal degrees)." ;
                                              rdfs:isDefinedBy "http://www.w3.org/2003/01/geo/wgs84_pos" ;
                                              rdfs:label "latitude" .


###  http://www.w3.org/2003/01/geo/wgs84_pos#long
<http://www.w3.org/2003/01/geo/wgs84_pos#long> rdf:type owl:DatatypeProperty ;
                                               rdfs:domain <http://www.w3.org/2003/01/geo/wgs84_pos#SpatialThing> ;
                                               rdfs:comment "The WGS84 longitude of a SpatialThing (decimal degrees)." ;
                                               rdfs:isDefinedBy "http://www.w3.org/2003/01/geo/wgs84_pos" ;
                                               rdfs:label "longitude" .


###  http://www.w3.org/2006/time#inXSDDateTimeStamp
time:inXSDDateTimeStamp rdf:type owl:DatatypeProperty ;
                        rdfs:domain time:Instant ;
                        rdfs:range xsd:dateTimeStamp ;
                        rdfs:comment "Position of an instant, expressed using xsd:dateTimeStamp" ;
                        rdfs:isDefinedBy "http://www.w3.org/2006/time" ;
                        rdfs:label "inXSDDateTimeStamp"@en .


###  https://saref.etsi.org/core/hasTimestamp
saref:hasTimestamp rdf:type owl:DatatypeProperty ;
                   rdfs:comment "A relationship stating the timestamp of an entity (e.g. a measurement)."@en ;
                   rdfs:isDefinedBy <https://saref.etsi.org/core> ;
                   rdfs:label "has timestamp"@en .


###  https://saref.etsi.org/core/hasValue
saref:hasValue rdf:type owl:DatatypeProperty ;
               rdfs:domain s4auto:OWLClass_553f9409_f262_4ed9_a940_180eb68bbb2a ;
               rdfs:range xsd:float ;
               rdfs:comment <https://saref.etsi.org/core> ,
                            "A relationship defining the value of a certain property, e.g., energy or power. Note that, even if numeric values are expected to enable reasoning, measurement values could use other datatypes."@en ;
               rdfs:label "has value"@en .


###  https://saref.etsi.org/saref4auto/OWLDataProperty_60a77575_e39d_454c_96c5_66f14035eb2e
s4auto:OWLDataProperty_60a77575_e39d_454c_96c5_66f14035eb2e rdf:type owl:DatatypeProperty ;
                                                            rdfs:domain s4auto:OWLClass_553f9409_f262_4ed9_a940_180eb68bbb2a ;
                                                            rdfs:range xsd:string ;
                                                            rdfs:label "hasOwner"@es .


###  https://saref.etsi.org/saref4auto/OWLDataProperty_f859b87a_028e_46d7_a87e_d75bf80fe7c7
s4auto:OWLDataProperty_f859b87a_028e_46d7_a87e_d75bf80fe7c7 rdf:type owl:DatatypeProperty ;
                                                            rdfs:domain s4auto:OWLClass_553f9409_f262_4ed9_a940_180eb68bbb2a ;
                                                            rdfs:range xsd:string ;
                                                            rdfs:label "hasProvider"@es .


###  https://saref.etsi.org/saref4auto/hasConfidenceValue
s4auto:hasConfidenceValue rdf:type owl:DatatypeProperty ;
                          rdfs:comment "A relation between the confidence (s4auto:Confidence) and its value, which can be a discrete value (+/- 5 cm/s) or a level (e.g. 95 %)"@en ;
                          rdfs:label "hasConfidenceValue"@en .


###  https://saref.etsi.org/saref4auto/hasCoordinateX
s4auto:hasCoordinateX rdf:type owl:DatatypeProperty ;
                      rdfs:comment "A relation to define the X coordinate of a relative position"@en ;
                      rdfs:label "hasCoordinateX"@en .


###  https://saref.etsi.org/saref4auto/hasCoordinateY
s4auto:hasCoordinateY rdf:type owl:DatatypeProperty ;
                      rdfs:comment "A relation to define the Y coordinate of a relative position"@en ;
                      rdfs:label "hasCoordinateY"@en .


###  https://saref.etsi.org/saref4auto/hasCoordinateZ
s4auto:hasCoordinateZ rdf:type owl:DatatypeProperty ;
                      rdfs:comment "A relation to define the Z coordinate of a relative position"@en ;
                      rdfs:label "hasCoordinateY"@en .


###  https://saref.etsi.org/saref4auto/hasDescriptionName
s4auto:hasDescriptionName rdf:type owl:DatatypeProperty ;
                          rdfs:comment "A relation to define that a parking spot can have a description name"@en ;
                          rdfs:label "hasDescriptionName"@en .


###  https://saref.etsi.org/saref4auto/hasEstimatedJoiningTime
s4auto:hasEstimatedJoiningTime rdf:type owl:DatatypeProperty ;
                               rdfs:range xsd:dateTime ;
                               rdfs:comment "A relation to express that, during the forming state, a vehicle member of a platoon is given an estimated time for joining" ;
                               rdfs:label "hasEstimatedJoiningTime"@en .


###  https://saref.etsi.org/saref4auto/hasIDValue
s4auto:hasIDValue rdf:type owl:DatatypeProperty ;
                  rdfs:comment "A relationship to define the value of an indentifier"@en ;
                  rdfs:label "hasIDValue"@en .


###  https://saref.etsi.org/saref4auto/hasMaxSize
s4auto:hasMaxSize rdf:type owl:DatatypeProperty ;
                  rdfs:comment "A relation to express the max size of a platoon. Note that it is defined as a datatype property as this is a fixed/static value of the platoon that does not change over time. In contrast, the current size of the platoon is actually a measurement that may change over time and it is therefore defined as an object property (see s4auto:hasSize)."@en ;
                  rdfs:label "hasMaxSize"@en .


###  https://saref.etsi.org/saref4auto/hasPlatoonIndex
s4auto:hasPlatoonIndex rdf:type owl:DatatypeProperty ;
                       rdfs:range xsd:int ;
                       rdfs:comment "A relation to express the index of the vehicle in the platoon starting from zero (leader) up to N (trailing vehicle)"@en ;
                       rdfs:label "hasPlatoonIndex"@en .


#################################################################
#    Classes
#################################################################

###  http://www.opengis.net/ont/geosparql#Feature
geosp:Feature rdf:type owl:Class ;
              rdfs:subClassOf geosp:SpatialObject ;
              owl:disjointWith geosp:Geometry ;
              rdfs:comment """This class represents the top-level feature type. This class is 
      equivalent to GFI_Feature defined in ISO 19156:2011, and it is 
      superclass of all feature types.""" ;
              rdfs:isDefinedBy <http://www.opengis.net/ont/geosparql> ;
              rdfs:label "Feature"@en .


###  http://www.opengis.net/ont/geosparql#Geometry
geosp:Geometry rdf:type owl:Class ;
               rdfs:subClassOf geosp:SpatialObject ;
               rdfs:comment """The class represents the top-level geometry type. This class is 
      equivalent to the UML class GM_Object defined in ISO 19107, and 
      it is superclass of all geometry types.""" ;
               rdfs:isDefinedBy <http://www.opengis.net/ont/geosparql> ;
               rdfs:label "Geometry"@en .


###  http://www.opengis.net/ont/geosparql#SpatialObject
geosp:SpatialObject rdf:type owl:Class ;
                    rdfs:comment """The class spatial-object represents everything that can have 
      a spatial representation. It is superclass of feature and geometry.""" ;
                    rdfs:isDefinedBy <http://www.opengis.net/ont/geosparql> ;
                    rdfs:label "SpatialObject"@en .


###  http://www.w3.org/2003/01/geo/wgs84_pos#Point
<http://www.w3.org/2003/01/geo/wgs84_pos#Point> rdf:type owl:Class ;
                                                rdfs:subClassOf <http://www.w3.org/2003/01/geo/wgs84_pos#SpatialThing> ;
                                                rdfs:comment "A point, typically described using a coordinate system relative to Earth, such as WGS84." ,
                                                             """Uniquely identified by lat/long/alt. i.e.

spaciallyIntersects(P1, P2) :- lat(P1, LAT), long(P1, LONG), alt(P1, ALT),
  lat(P2, LAT), long(P2, LONG), alt(P2, ALT).

sameThing(P1, P2) :- type(P1, Point), type(P2, Point), spaciallyIntersects(P1, P2).""" ;
                                                rdfs:isDefinedBy "http://www.w3.org/2003/01/geo/wgs84_pos#" ;
                                                rdfs:label "Point"@en .


###  http://www.w3.org/2003/01/geo/wgs84_pos#SpatialThing
<http://www.w3.org/2003/01/geo/wgs84_pos#SpatialThing> rdf:type owl:Class ;
                                                       rdfs:comment """Anything with spatial extent, i.e. size, shape, or position.
 e.g. people, places, bowling balls, as well as abstract areas like cubes.""" ;
                                                       rdfs:isDefinedBy "http://www.w3.org/2003/01/geo/wgs84_pos#" ;
                                                       rdfs:label "Spatial Thing"@en .


###  http://www.w3.org/2006/time#Instant
time:Instant rdf:type owl:Class ;
             rdfs:subClassOf time:TemporalEntity ;
             rdfs:comment "A temporal entity with zero extent or duration" ;
             rdfs:isDefinedBy "http://www.w3.org/2006/time" ;
             rdfs:label "Instant"@en .


###  http://www.w3.org/2006/time#Interval
time:Interval rdf:type owl:Class ;
              rdfs:subClassOf time:TemporalEntity ;
              rdfs:comment "A temporal entity with an extent or duration" ;
              rdfs:isDefinedBy "http://www.w3.org/2006/time" ;
              rdfs:label "Interval"@en .


###  http://www.w3.org/2006/time#TemporalEntity
time:TemporalEntity rdf:type owl:Class ;
                    rdfs:comment "A temporal interval or instant." ;
                    rdfs:isDefinedBy "http://www.w3.org/2006/time" ;
                    rdfs:label "TemporaryEntity"@en .


###  https://saref.etsi.org/core/Actuator
saref:Actuator rdf:type owl:Class ;
               rdfs:subClassOf saref:Device ;
               rdfs:comment "A device responsible for moving or controlling a mechanism or system."@en ;
               rdfs:isDefinedBy <https://saref.etsi.org/core> ;
               rdfs:label "Actuator"@en .


###  https://saref.etsi.org/core/Device
saref:Device rdf:type owl:Class ;
             rdfs:subClassOf [ rdf:type owl:Restriction ;
                               owl:onProperty saref:controlsProperty ;
                               owl:allValuesFrom saref:Property
                             ] ,
                             [ rdf:type owl:Restriction ;
                               owl:onProperty saref:makesMeasurement ;
                               owl:allValuesFrom saref:Measurement
                             ] ,
                             [ rdf:type owl:Restriction ;
                               owl:onProperty saref:measuresProperty ;
                               owl:allValuesFrom saref:Property
                             ] ;
             rdfs:comment "A tangible object designed to accomplish a particular task in households, common public buildings or offices. In order to accomplish this task, the device performs one or more functions. For example, a washing machine is designed to wash (task) and to accomplish this task it performs a start and stop function. Devices can be structured in categories (subclasses) that reflect the different domain in which a device is used, e.g., smart appliances domain (subclass FunctionRelated) vs. building domain (subclass BuildingRelated) vs. smart grid domain (subclass EnergyRelated). New categories can be defined,if needed, to reflect other differences, for example different points of view, such as the point of view of the device's user vs. the point of view of the device's manufacturer. We propose a list of devices that are relevant for the purpose of SAREF, but this list can be extended."@en ;
             rdfs:isDefinedBy saref: ;
             rdfs:label "Device"@en .


###  https://saref.etsi.org/core/FeatureOfInterest
saref:FeatureOfInterest rdf:type owl:Class ;
                        rdfs:subClassOf [ rdf:type owl:Restriction ;
                                          owl:onProperty s4auto:hasIdentifier ;
                                          owl:someValuesFrom s4auto:Identifier
                                        ] ,
                                        [ rdf:type owl:Restriction ;
                                          owl:onProperty saref:hasProperty ;
                                          owl:allValuesFrom saref:Property
                                        ] ;
                        rdfs:comment "A feature of interest represents any real world entity from which a property is measured."@en ;
                        rdfs:isDefinedBy saref: ;
                        rdfs:label "FeatureOfInterest"@en .


###  https://saref.etsi.org/core/Measurement
saref:Measurement rdf:type owl:Class ;
                  rdfs:subClassOf [ rdf:type owl:Restriction ;
                                    owl:onProperty saref:measurementMadeBy ;
                                    owl:someValuesFrom saref:Device
                                  ] ,
                                  [ rdf:type owl:Restriction ;
                                    owl:onProperty s4auto:hasConfidence ;
                                    owl:someValuesFrom s4auto:Confidence
                                  ] ,
                                  [ rdf:type owl:Restriction ;
                                    owl:onProperty saref:isMeasuredIn ;
                                    owl:allValuesFrom saref:UnitOfMeasure
                                  ] ,
                                  [ rdf:type owl:Restriction ;
                                    owl:onProperty saref:relatesToProperty ;
                                    owl:allValuesFrom saref:Property
                                  ] ,
                                  [ rdf:type owl:Restriction ;
                                    owl:onProperty saref:isMeasuredIn ;
                                    owl:qualifiedCardinality "1"^^xsd:nonNegativeInteger ;
                                    owl:onClass saref:UnitOfMeasure
                                  ] ,
                                  [ rdf:type owl:Restriction ;
                                    owl:onProperty saref:relatesToProperty ;
                                    owl:qualifiedCardinality "1"^^xsd:nonNegativeInteger ;
                                    owl:onClass saref:Property
                                  ] ,
                                  [ rdf:type owl:Restriction ;
                                    owl:onProperty saref:hasTimestamp ;
                                    owl:allValuesFrom xsd:dateTime
                                  ] ,
                                  [ rdf:type owl:Restriction ;
                                    owl:onProperty saref:hasValue ;
                                    owl:qualifiedCardinality "1"^^xsd:nonNegativeInteger ;
                                    owl:onDataRange xsd:float
                                  ] ;
                  rdfs:comment "Represents the measured value made over a property. It is also linked to the unit of measure in which the value is expressed and the timestamp of the measurement."@en ;
                  rdfs:isDefinedBy saref: ;
                  rdfs:label "Measurement"@en .


###  https://saref.etsi.org/core/Property
saref:Property rdf:type owl:Class ;
               rdfs:subClassOf [ rdf:type owl:Restriction ;
                                 owl:onProperty saref:isControlledByDevice ;
                                 owl:allValuesFrom saref:Device
                               ] ,
                               [ rdf:type owl:Restriction ;
                                 owl:onProperty saref:isMeasuredByDevice ;
                                 owl:allValuesFrom saref:Device
                               ] ,
                               [ rdf:type owl:Restriction ;
                                 owl:onProperty saref:relatesToMeasurement ;
                                 owl:allValuesFrom saref:Measurement
                               ] ;
               rdfs:comment "Anything that can be sensed, measured or controlled by a device (measured by a sensor, controlled by an actuator) ."@en ;
               rdfs:isDefinedBy <https://saref.etsi.org/core> ;
               rdfs:label "Property"@en .


###  https://saref.etsi.org/core/Sensor
saref:Sensor rdf:type owl:Class ;
             rdfs:subClassOf saref:Device ;
             rdfs:comment "A device that detects and responds to events or changes in the physical environment such as light, motion, or temperature changes. A device that has category saref:Sensor and performs a saref:SensingFunction."@en ;
             rdfs:isDefinedBy <https://saref.etsi.org/core> ;
             rdfs:label "Sensor"@en .


###  https://saref.etsi.org/core/State
saref:State rdf:type owl:Class ;
            rdfs:comment "The state in which a device can be found, e.g, ON/OFF/STANDBY, or ONLINE/OFFLINE. We propose here a list of states that are relevant for the purpose of SAREF, but this list can be extended."@en ;
            rdfs:isDefinedBy <https://saref.etsi.org/core> ;
            rdfs:label "State"@en .


###  https://saref.etsi.org/core/UnitOfMeasure
saref:UnitOfMeasure rdf:type owl:Class ;
                    rdfs:comment "The unit of measure is a standard for measurement of a quantity, such as a Property. For example, Power is a property and Watt is a unit of power that represents a definite predetermined power: when we say 10 Watt, we actually mean 10 times the definite predetermined power called \"watt\". Our definition is based on the definition of unit of measure in the Ontology of units of Measure (OM). We propose here a list of some units of measure that are relevant for the purpose of SAREF, but this list can be extended, also using some other ontologies rather than the Ontology of units of Measure (OM)."@en ;
                    rdfs:isDefinedBy saref: ;
                    rdfs:label "UnitOfMeasure"@en .


###  https://saref.etsi.org/saref4auto/AbsolutePosition
s4auto:AbsolutePosition rdf:type owl:Class ;
                        rdfs:subClassOf s4auto:Point ,
                                        s4auto:Position ,
                                        [ rdf:type owl:Restriction ;
                                          owl:onProperty s4auto:hasAbsolutePosition ;
                                          owl:someValuesFrom s4auto:AbsolutePosition
                                        ] ,
                                        [ rdf:type owl:Restriction ;
                                          owl:onProperty <http://www.w3.org/2003/01/geo/wgs84_pos#alt> ;
                                          owl:someValuesFrom xsd:float
                                        ] ,
                                        [ rdf:type owl:Restriction ;
                                          owl:onProperty <http://www.w3.org/2003/01/geo/wgs84_pos#lat> ;
                                          owl:someValuesFrom xsd:float
                                        ] ,
                                        [ rdf:type owl:Restriction ;
                                          owl:onProperty <http://www.w3.org/2003/01/geo/wgs84_pos#long> ;
                                          owl:someValuesFrom xsd:float
                                        ] ;
                        rdfs:comment "The absolute poistion of an automotive object in terms of lat, long and lat"@en ;
                        rdfs:label "AbsolutePosition"@en .


###  https://saref.etsi.org/saref4auto/AbsoluteSpeed
s4auto:AbsoluteSpeed rdf:type owl:Class ;
                     rdfs:subClassOf s4auto:Speed ;
                     rdfs:comment "A type of speed"@en ;
                     rdfs:label "AbsoluteSpeed"@en .


###  https://saref.etsi.org/saref4auto/Acceleration
s4auto:Acceleration rdf:type owl:Class ;
                    rdfs:subClassOf saref:Property ,
                                    [ rdf:type owl:Restriction ;
                                      owl:onProperty saref:isMeasuredIn ;
                                      owl:allValuesFrom s4auto:OWLClass_9ffbba79_32b5_41e3_9f34_6d82b4c49fe0
                                    ] ,
                                    [ rdf:type owl:Restriction ;
                                      owl:onProperty saref:hasValue ;
                                      owl:someValuesFrom xsd:float
                                    ] ;
                    rdfs:comment "A Property of interest for the automotive domain"@en ;
                    rdfs:label "Acceleration"@en .


###  https://saref.etsi.org/saref4auto/AccelerationConfidence
s4auto:AccelerationConfidence rdf:type owl:Class ;
                              rdfs:subClassOf s4auto:Confidence ,
                                              [ rdf:type owl:Restriction ;
                                                owl:onProperty s4auto:hasConfidenceValue ;
                                                owl:someValuesFrom xsd:float
                                              ] ;
                              rdfs:comment "A type of confidence for acceleration measurements that represents the absolute accuracy of a reported vehicle acceleration value with a predefined confidence level (e.g. 95 %)"@en ;
                              rdfs:label "AccelerationConfidence"@en .


###  https://saref.etsi.org/saref4auto/Address
s4auto:Address rdf:type owl:Class ;
               rdfs:comment "A class to define common information related to an address. It is out of scope of SAREF4AUTO to define the details of such an address. It is instead recommended to reuse existing ontologies that specify how to model an address in terms of Street, Postal Code, City, Region, Country, etc."@en ;
               rdfs:label "Address"@en .


###  https://saref.etsi.org/saref4auto/AngularDirection
s4auto:AngularDirection rdf:type owl:Class ;
                        rdfs:subClassOf s4auto:Heading ;
                        rdfs:comment "A type of heading"@en ;
                        rdfs:label "AngularDirection"@en .


###  https://saref.etsi.org/saref4auto/Assembling
s4auto:Assembling rdf:type owl:Class ;
                  rdfs:subClassOf s4auto:PlatoonState ;
                  rdfs:comment "A type of state for Platoon"@en ;
                  rdfs:label "assembling"@en .


###  https://saref.etsi.org/saref4auto/AtDropOffSpot
s4auto:AtDropOffSpot rdf:type owl:Class ;
                     rdfs:subClassOf s4auto:ParkingVehicleState ;
                     rdfs:comment "A type of state for Parking Vehicle"@en ;
                     rdfs:label "At Drop Off Spot"@en .


###  https://saref.etsi.org/saref4auto/AtPickUpSpot
s4auto:AtPickUpSpot rdf:type owl:Class ;
                    rdfs:subClassOf s4auto:ParkingVehicleState ;
                    rdfs:comment "A type of state for Parking Vehicle"@en ;
                    rdfs:label "At Pick Up Spot"@en .


###  https://saref.etsi.org/saref4auto/AutomationLevel
s4auto:AutomationLevel rdf:type owl:Class ;
                       rdfs:comment "The level of automation a platoon of vehicles or a singular vehicle"@en ;
                       rdfs:label "AutomationLevel"@en .


###  https://saref.etsi.org/saref4auto/AutomotiveObject
s4auto:AutomotiveObject rdf:type owl:Class ;
                        rdfs:comment "The main objects of interest in the automotive domain."@en ;
                        rdfs:label "AutomotiveObject"@en .


###  https://saref.etsi.org/saref4auto/BrakeCapacity
s4auto:BrakeCapacity rdf:type owl:Class ;
                     rdfs:subClassOf saref:Property ;
                     rdfs:comment "A Property of interest for the automotive domain"@en ;
                     rdfs:label "BrakeCapacity"@en .


###  https://saref.etsi.org/saref4auto/Bus
s4auto:Bus rdf:type owl:Class ;
           rdfs:subClassOf s4auto:PublicTransport ;
           rdfs:comment "A type of public transport"@en ;
           rdfs:label "Bus"@en .


###  https://saref.etsi.org/saref4auto/Car
s4auto:Car rdf:type owl:Class ;
           rdfs:subClassOf s4auto:Vehicle ;
           rdfs:comment "A type of vehicle. Example of a car is a passenger car"@en ;
           rdfs:label "Car"@en .


###  https://saref.etsi.org/saref4auto/CardinalityUnit
s4auto:CardinalityUnit rdf:type owl:Class ;
                       rdfs:subClassOf saref:UnitOfMeasure ;
                       rdfs:comment "unit of measure of size"@en ;
                       rdfs:label "cardinality unit"@en .


###  https://saref.etsi.org/saref4auto/Charging
s4auto:Charging rdf:type owl:Class ;
                rdfs:subClassOf s4auto:ParkingSpotState ,
                                s4auto:ParkingVehicleState ;
                rdfs:comment "A type of state for Parking Spot or for Parking Vehicle"@en ;
                rdfs:label "charging"@en .


###  https://saref.etsi.org/saref4auto/Closed
s4auto:Closed rdf:type owl:Class ;
              rdfs:subClassOf s4auto:ParkingSpotState ;
              rdfs:comment "A type of state for Parking Spot"@en ;
              rdfs:label "closed"@en .


###  https://saref.etsi.org/saref4auto/Confidence
s4auto:Confidence rdf:type owl:Class ;
                  rdfs:subClassOf [ rdf:type owl:Restriction ;
                                    owl:onProperty s4auto:hasConfidenceUnitOfMeasure ;
                                    owl:someValuesFrom saref:UnitOfMeasure
                                  ] ,
                                  [ rdf:type owl:Restriction ;
                                    owl:onProperty s4auto:hasConfidenceValue ;
                                    owl:someValuesFrom xsd:float
                                  ] ;
                  rdfs:comment "Every measurement in the automotive domain is an estimated measurement coming from the aggregation of several measurements from different sensor or devices taken at the same time or at consecutive times very close to each other. Therefore, a confidence is always associated to each mesurement to indicate that it has not 100% accuracy."@en ;
                  rdfs:label "Confidence"@en .


###  https://saref.etsi.org/saref4auto/CriticalObject
s4auto:CriticalObject rdf:type owl:Class ;
                      rdfs:subClassOf owl:Thing ,
                                      [ rdf:type owl:Restriction ;
                                        owl:onProperty s4auto:hasHeight ;
                                        owl:someValuesFrom s4auto:Height
                                      ] ,
                                      [ rdf:type owl:Restriction ;
                                        owl:onProperty s4auto:hasLength ;
                                        owl:someValuesFrom s4auto:Length
                                      ] ,
                                      [ rdf:type owl:Restriction ;
                                        owl:onProperty s4auto:hasMovement ;
                                        owl:someValuesFrom s4auto:Movement
                                      ] ,
                                      [ rdf:type owl:Restriction ;
                                        owl:onProperty s4auto:hasShape ;
                                        owl:someValuesFrom s4auto:Shape
                                      ] ,
                                      [ rdf:type owl:Restriction ;
                                        owl:onProperty s4auto:hasWidth ;
                                        owl:someValuesFrom s4auto:Width
                                      ] ;
                      rdfs:comment "A critical object located on the road. Critical objects are small object, medium object, large object"@en ;
                      rdfs:label "CriticalObject"@en .


###  https://saref.etsi.org/saref4auto/Disengaging
s4auto:Disengaging rdf:type owl:Class ;
                   rdfs:subClassOf s4auto:PlatoonState ,
                                   s4auto:PlatoonVehicleState ;
                   rdfs:comment "A type of state for Platoon or for a Vehicle in a Platoon"@en ;
                   rdfs:label "disengaging"@en .


###  https://saref.etsi.org/saref4auto/DrivingToParkingSpot
s4auto:DrivingToParkingSpot rdf:type owl:Class ;
                            rdfs:subClassOf s4auto:ParkingVehicleState ;
                            rdfs:comment "A type of state for Parking Vehicle"@en ;
                            rdfs:label "Driving To Parking Spot"@en .


###  https://saref.etsi.org/saref4auto/DrivingToPickUpSpot
s4auto:DrivingToPickUpSpot rdf:type owl:Class ;
                           rdfs:subClassOf s4auto:ParkingVehicleState ;
                           rdfs:comment "A type of state for Parking Vehicle"@en ;
                           rdfs:label "Driving To Pick Up Spot"@en .


###  https://saref.etsi.org/saref4auto/ElectricChargingParkingSpot
s4auto:ElectricChargingParkingSpot rdf:type owl:Class ;
                                   rdfs:subClassOf s4auto:ParkingSpot ;
                                   rdfs:comment "A type pf parking spot"@en ;
                                   rdfs:label "ElectricChargingParkingSpot"@en .


###  https://saref.etsi.org/saref4auto/ElectronicControlUnit
s4auto:ElectronicControlUnit rdf:type owl:Class ;
                             rdfs:subClassOf saref:Device ,
                                             s4syst:System ,
                                             [ rdf:type owl:Restriction ;
                                               owl:onProperty saref:measuresProperty ;
                                               owl:someValuesFrom s4auto:Acceleration
                                             ] ,
                                             [ rdf:type owl:Restriction ;
                                               owl:onProperty saref:measuresProperty ;
                                               owl:someValuesFrom s4auto:Heading
                                             ] ,
                                             [ rdf:type owl:Restriction ;
                                               owl:onProperty saref:measuresProperty ;
                                               owl:someValuesFrom s4auto:Speed
                                             ] ,
                                             [ rdf:type owl:Restriction ;
                                               owl:onProperty s4auto:detectsPosition ;
                                               owl:someValuesFrom s4auto:Position
                                             ] ,
                                             [ rdf:type owl:Restriction ;
                                               owl:onProperty s4auto:usesMeasurement ;
                                               owl:someValuesFrom saref:Measurement
                                             ] ,
                                             [ rdf:type owl:Restriction ;
                                               owl:onProperty s4syst:subSystemOf ;
                                               owl:someValuesFrom s4auto:Vehicle
                                             ] ;
                             rdfs:comment "An electronic control unit (ECU) is any embedded system in automotive electronics that monitors and controls one or more of the electrical systems or subsystems in a vehicle. The ECU provides measurements about relevant properties of the vehicle, such as speed, acceleration, position, etc."@en ;
                             rdfs:label "ElectronicControlUnit"@en .


###  https://saref.etsi.org/saref4auto/EndPoint
s4auto:EndPoint rdf:type owl:Class ;
                rdfs:subClassOf s4auto:Point ;
                rdfs:comment "The final destination of a vehicle or a platoon, or the final point of a route"@en ;
                rdfs:label "EndPoint"@en .


###  https://saref.etsi.org/saref4auto/Engaging
s4auto:Engaging rdf:type owl:Class ;
                rdfs:subClassOf s4auto:PlatoonVehicleState ;
                rdfs:comment "A type of state for a Vehicle in a Platoon"@en ;
                rdfs:label "engaging"@en .


###  https://saref.etsi.org/saref4auto/Forming
s4auto:Forming rdf:type owl:Class ;
               rdfs:subClassOf s4auto:PlatoonVehicleState ;
               rdfs:comment "A type of state for a Vehicle in a Platoon"@en ;
               rdfs:label "forming"@en .


###  https://saref.etsi.org/saref4auto/Free
s4auto:Free rdf:type owl:Class ;
            rdfs:subClassOf s4auto:ParkingSpotState ;
            rdfs:comment "A type of state for Parking Spot"@en ;
            rdfs:label "free"@en .


###  https://saref.etsi.org/saref4auto/Heading
s4auto:Heading rdf:type owl:Class ;
               rdfs:subClassOf saref:Property ;
               rdfs:comment "A Property of interest for the automotive domain"@en ;
               rdfs:label "Heading"@en .


###  https://saref.etsi.org/saref4auto/HeavyTruck
s4auto:HeavyTruck rdf:type owl:Class ;
                  rdfs:subClassOf s4auto:Truck ;
                  rdfs:comment "A type of truck"@en ;
                  rdfs:label "HeavyTruck"@en .


###  https://saref.etsi.org/saref4auto/Height
s4auto:Height rdf:type owl:Class ;
              rdfs:subClassOf saref:Property ,
                              [ rdf:type owl:Restriction ;
                                owl:onProperty saref:isMeasuredIn ;
                                owl:allValuesFrom s4auto:HeightUnit
                              ] ,
                              [ rdf:type owl:Restriction ;
                                owl:onProperty saref:hasValue ;
                                owl:someValuesFrom xsd:float
                              ] ;
              rdfs:comment "A Property of interest for the automotive domain"@en ;
              rdfs:label "Height"@en .


###  https://saref.etsi.org/saref4auto/HeightUnit
s4auto:HeightUnit rdf:type owl:Class ;
                  rdfs:subClassOf saref:UnitOfMeasure ;
                  rdfs:comment "unit of measure of height"@en ;
                  rdfs:label "height unit"@en .


###  https://saref.etsi.org/saref4auto/Identifier
s4auto:Identifier rdf:type owl:Class ;
                  rdfs:subClassOf [ rdf:type owl:Restriction ;
                                    owl:onProperty s4auto:hasIDValue ;
                                    owl:someValuesFrom xsd:string
                                  ] ;
                  rdfs:comment "A class used to identify 1)  a vehicle (station) during data exchange with other devices/stations 2) a platoon during data exchange with other devices/stations, 3)  a parking spot within a parking area during data exchange with other devices/stations. In all cases, this identifier may be a pseudonym. It may change over space and/or over time."@en ;
                  rdfs:label "Identifier"@en .


###  https://saref.etsi.org/saref4auto/LargeObject
s4auto:LargeObject rdf:type owl:Class ;
                   rdfs:subClassOf s4auto:CriticalObject ;
                   rdfs:comment "A type of Critical Object"@en ;
                   rdfs:label "Large Object"@en .


###  https://saref.etsi.org/saref4auto/LateralAcceleration
s4auto:LateralAcceleration rdf:type owl:Class ;
                           rdfs:subClassOf s4auto:Acceleration ;
                           rdfs:comment "A type of acceleration"@en ;
                           rdfs:label "Lateral Acceleration"@en .


###  https://saref.etsi.org/saref4auto/Length
s4auto:Length rdf:type owl:Class ;
              rdfs:subClassOf saref:Property ,
                              [ rdf:type owl:Restriction ;
                                owl:onProperty saref:isMeasuredIn ;
                                owl:allValuesFrom s4auto:LengthUnit
                              ] ,
                              [ rdf:type owl:Restriction ;
                                owl:onProperty saref:hasValue ;
                                owl:someValuesFrom xsd:float
                              ] ;
              rdfs:comment "A Property of interest for the automotive domain"@en ,
                           "In a platoon, a property to express that a platoon has a size. This size is defined as 1) the total number of vehicles currently in the platoon (see s4auto:Size class); or 2) Length of the platoon (sum of all vehicles' length + inter-vehicle distance)"@en ;
              rdfs:label "Length"@en .


###  https://saref.etsi.org/saref4auto/LengthUnit
s4auto:LengthUnit rdf:type owl:Class ;
                  rdfs:subClassOf saref:UnitOfMeasure ;
                  rdfs:comment "unit of measure of lenght"@en ;
                  rdfs:label "length unit"@en .


###  https://saref.etsi.org/saref4auto/LightTruck
s4auto:LightTruck rdf:type owl:Class ;
                  rdfs:subClassOf s4auto:Truck ;
                  rdfs:comment "A type of truck"@en ;
                  rdfs:label "LightTruck"@en .


###  https://saref.etsi.org/saref4auto/LongitudinalAcceleration
s4auto:LongitudinalAcceleration rdf:type owl:Class ;
                                rdfs:subClassOf s4auto:Acceleration ;
                                rdfs:comment "A type of acceleration"@en ;
                                rdfs:label "LongitudinalAcceleration"@en .


###  https://saref.etsi.org/saref4auto/MediumObject
s4auto:MediumObject rdf:type owl:Class ;
                    rdfs:subClassOf s4auto:CriticalObject ;
                    rdfs:comment "A type of Critical Object"@en ;
                    rdfs:label "Medium Object"@en .


###  https://saref.etsi.org/saref4auto/Movement
s4auto:Movement rdf:type owl:Class ;
                rdfs:subClassOf saref:Property ;
                rdfs:comment "A Property of interest for the automotive domain. Relevant types of movement are: Static (position only), moving in same direction (speed, acceleration), moving in reverse direction (speed acceleration), crossing (speed, acceleration, direction)"@en ;
                rdfs:label "Movement"@en .


###  https://saref.etsi.org/saref4auto/NotifiedEvent
s4auto:NotifiedEvent rdf:type owl:Class ;
                     rdfs:subClassOf owl:Thing ;
                     rdfs:comment "The relevant types of events are trafficCondition, accident, roadworks, impassability, adverseWeatherCondition-Adhesion, aquaplannning, hazardousLocation-SurfaceCondition, hazardousLocation-ObstacleOnTheRoad, hazardousLocation-AnimalOnTheRoad, humanPresenceOnTheRoad, wrongWayDriving, rescueAndRecoveryWorkInProgress, adverseWeatherCondition-ExtremeWeatherCondition, adverseWeatherCondition-Visibility, adverseWeatherCondition-Precipitation, slowVehicle, dangerousEndOfQueue, vehicleBreakdown, postCrash, humanProblem, stationaryVehicle, emergencyVehicleApproaching, hazardousLocation-DangerousCurve, collisionRisk, signalViolation, dangerousSituation"@en ;
                     rdfs:label "NotifiedEvent"@en .


###  https://saref.etsi.org/saref4auto/OWLClass_083fab3f_ca95_4af8_873e_7563bd6bec77
s4auto:OWLClass_083fab3f_ca95_4af8_873e_7563bd6bec77 rdf:type owl:Class ;
                                                     rdfs:subClassOf s4auto:OWLClass_d2f64388_08b5_4626_8be5_bf2614562bb8 ,
                                                                     [ rdf:type owl:Restriction ;
                                                                       owl:onProperty s4auto:OWLObjectProperty_c016f3d4_1a3a_4a8b_b22d_56aaff72f689 ;
                                                                       owl:someValuesFrom saref:Property
                                                                     ] ;
                                                     rdfs:label "Historic_data"@es .


###  https://saref.etsi.org/saref4auto/OWLClass_094f68a1_a622_4a62_9298_43b74210b8a4
s4auto:OWLClass_094f68a1_a622_4a62_9298_43b74210b8a4 rdf:type owl:Class ;
                                                     rdfs:subClassOf s4auto:OWLClass_268735bf_d97b_43a0_80f7_ead69c3861fa ,
                                                                     [ rdf:type owl:Restriction ;
                                                                       owl:onProperty s4auto:OWLObjectProperty_1828ea5b_6175_4e01_88e4_a1b9cab3b318 ;
                                                                       owl:someValuesFrom s4auto:Vehicle
                                                                     ] ;
                                                     owl:disjointWith s4auto:OWLClass_8b969e76_5374_4dc6_a45d_f32e5769cafa ;
                                                     rdfs:label "Public_transport_data"@es .


###  https://saref.etsi.org/saref4auto/OWLClass_0f32b2d8_db89_4881_ace7_72cace8ba5de
s4auto:OWLClass_0f32b2d8_db89_4881_ace7_72cace8ba5de rdf:type owl:Class ;
                                                     rdfs:subClassOf saref:Property ,
                                                                     [ rdf:type owl:Restriction ;
                                                                       owl:onProperty saref:isMeasuredIn ;
                                                                       owl:allValuesFrom s4auto:OWLClass_7227c333_67f8_4f2d_a0e1_208d15683bb5
                                                                     ] ,
                                                                     [ rdf:type owl:Restriction ;
                                                                       owl:onProperty saref:hasValue ;
                                                                       owl:someValuesFrom xsd:float
                                                                     ] ;
                                                     rdfs:comment "Property of interest. Flow of vehicle or people in a specific point" ;
                                                     rdfs:label "Flow"@es .


###  https://saref.etsi.org/saref4auto/OWLClass_1c2e7359_7ebf_4f4c_b511_6d579bc168fd
s4auto:OWLClass_1c2e7359_7ebf_4f4c_b511_6d579bc168fd rdf:type owl:Class ;
                                                     rdfs:subClassOf s4auto:OWLClass_094f68a1_a622_4a62_9298_43b74210b8a4 ;
                                                     rdfs:label "Timetable_of_simulation_period_data"@es .


###  https://saref.etsi.org/saref4auto/OWLClass_268735bf_d97b_43a0_80f7_ead69c3861fa
s4auto:OWLClass_268735bf_d97b_43a0_80f7_ead69c3861fa rdf:type owl:Class ;
                                                     rdfs:subClassOf s4auto:OWLClass_553f9409_f262_4ed9_a940_180eb68bbb2a ,
                                                                     [ rdf:type owl:Restriction ;
                                                                       owl:onProperty s4auto:OWLObjectProperty_10d4f71b_6da1_4eb5_840c_760db83f999d ;
                                                                       owl:someValuesFrom s4auto:OWLClass_836b22f0_3931_44dd_a18b_4f52f5d10379
                                                                     ] ,
                                                                     [ rdf:type owl:Restriction ;
                                                                       owl:onProperty s4auto:OWLObjectProperty_e1bbccf3_d604_4a6c_a130_e2148e0787fc ;
                                                                       owl:allValuesFrom s4auto:OWLClass_30dd4a6b_a368_45c4_bcb0_b2d8300ba2c1
                                                                     ] ,
                                                                     [ rdf:type owl:Restriction ;
                                                                       owl:onProperty s4auto:OWLDataProperty_60a77575_e39d_454c_96c5_66f14035eb2e ;
                                                                       owl:someValuesFrom xsd:string
                                                                     ] ,
                                                                     [ rdf:type owl:Restriction ;
                                                                       owl:onProperty s4auto:OWLDataProperty_f859b87a_028e_46d7_a87e_d75bf80fe7c7 ;
                                                                       owl:someValuesFrom xsd:string
                                                                     ] ;
                                                     rdfs:label "Transport_data"@es .


###  https://saref.etsi.org/saref4auto/OWLClass_28157908_14ae_4cbc_909d_850da3c26f2e
s4auto:OWLClass_28157908_14ae_4cbc_909d_850da3c26f2e rdf:type owl:Class ;
                                                     rdfs:subClassOf s4auto:OWLClass_8b969e76_5374_4dc6_a45d_f32e5769cafa ;
                                                     rdfs:comment "GIS shapefile of TAZ system and georeferences of centroids and connectors" ;
                                                     rdfs:label "TAZ_system_data"@es .


###  https://saref.etsi.org/saref4auto/OWLClass_2cc57115_7965_4f13_9ad6_139fbf337b2e
s4auto:OWLClass_2cc57115_7965_4f13_9ad6_139fbf337b2e rdf:type owl:Class ;
                                                     rdfs:subClassOf s4auto:OWLClass_f12ac0e6_d518_41b2_a737_112009debde8 ;
                                                     owl:disjointWith s4auto:OWLClass_be6b198e_5792_4367_8dd0_e1193127a9d0 ;
                                                     rdfs:label "Duration"@es .


###  https://saref.etsi.org/saref4auto/OWLClass_30dd4a6b_a368_45c4_bcb0_b2d8300ba2c1
s4auto:OWLClass_30dd4a6b_a368_45c4_bcb0_b2d8300ba2c1 rdf:type owl:Class ;
                                                     rdfs:subClassOf s4auto:OWLClass_553f9409_f262_4ed9_a940_180eb68bbb2a ;
                                                     rdfs:label "Adquisition_rate"@es .


###  https://saref.etsi.org/saref4auto/OWLClass_33be815d_25bd_48d7_bdb4_8a6febb58d2c
s4auto:OWLClass_33be815d_25bd_48d7_bdb4_8a6febb58d2c rdf:type owl:Class ;
                                                     rdfs:subClassOf s4auto:OWLClass_094f68a1_a622_4a62_9298_43b74210b8a4 ,
                                                                     [ rdf:type owl:Restriction ;
                                                                       owl:onProperty s4auto:hasAbsolutePosition ;
                                                                       owl:someValuesFrom s4auto:AbsolutePosition
                                                                     ] ;
                                                     rdfs:label "Stops_location_data"@es .


###  https://saref.etsi.org/saref4auto/OWLClass_38f0cbf1_e069_4e64_9812_7f81eac96690
s4auto:OWLClass_38f0cbf1_e069_4e64_9812_7f81eac96690 rdf:type owl:Class ;
                                                     rdfs:subClassOf s4auto:OWLClass_f2f0f1ca_8879_4599_8acf_34fcb5e0c2a6 ,
                                                                     [ rdf:type owl:Restriction ;
                                                                       owl:onProperty <http://www.w3.org/2003/01/geo/wgs84_pos#location> ;
                                                                       owl:allValuesFrom s4auto:Address
                                                                     ] ,
                                                                     [ rdf:type owl:Restriction ;
                                                                       owl:onProperty s4auto:OWLObjectProperty_e1bbccf3_d604_4a6c_a130_e2148e0787fc ;
                                                                       owl:allValuesFrom s4auto:OWLClass_083fab3f_ca95_4af8_873e_7563bd6bec77
                                                                     ] ,
                                                                     [ rdf:type owl:Restriction ;
                                                                       owl:onProperty s4auto:OWLObjectProperty_e1bbccf3_d604_4a6c_a130_e2148e0787fc ;
                                                                       owl:allValuesFrom s4auto:OWLClass_8ef04dbb_f94e_4dae_8bf0_cb63cd807909
                                                                     ] ;
                                                     rdfs:label "Antwerp_pilot"@es .


###  https://saref.etsi.org/saref4auto/OWLClass_3c89eac0_be9e_4296_ae63_6b28ca4f810b
s4auto:OWLClass_3c89eac0_be9e_4296_ae63_6b28ca4f810b rdf:type owl:Class ;
                                                     rdfs:subClassOf s4auto:OWLClass_094f68a1_a622_4a62_9298_43b74210b8a4 ;
                                                     rdfs:label "Stops_per_line_data"@es .


###  https://saref.etsi.org/saref4auto/OWLClass_3ef5abd6_4002_4095_96dd_008e5780e633
s4auto:OWLClass_3ef5abd6_4002_4095_96dd_008e5780e633 rdf:type owl:Class ;
                                                     rdfs:subClassOf s4auto:OWLClass_836b22f0_3931_44dd_a18b_4f52f5d10379 ;
                                                     rdfs:label "Shapefile"@es .


###  https://saref.etsi.org/saref4auto/OWLClass_495b7639_fa49_44c2_a634_3838926ad786
s4auto:OWLClass_495b7639_fa49_44c2_a634_3838926ad786 rdf:type owl:Class ;
                                                     rdfs:subClassOf s4auto:OWLClass_836b22f0_3931_44dd_a18b_4f52f5d10379 ;
                                                     rdfs:label "XLS"@es .


###  https://saref.etsi.org/saref4auto/OWLClass_553f9409_f262_4ed9_a940_180eb68bbb2a
s4auto:OWLClass_553f9409_f262_4ed9_a940_180eb68bbb2a rdf:type owl:Class ;
                                                     rdfs:label "Mobility_data"@es .


###  https://saref.etsi.org/saref4auto/OWLClass_62ab1c22_189c_4445_85ee_1ef1e2d17b57
s4auto:OWLClass_62ab1c22_189c_4445_85ee_1ef1e2d17b57 rdf:type owl:Class ;
                                                     rdfs:subClassOf s4auto:OWLClass_836b22f0_3931_44dd_a18b_4f52f5d10379 ;
                                                     rdfs:label "JSON"@es .


###  https://saref.etsi.org/saref4auto/OWLClass_6b9849f8_eb6a_4b0d_b135_c271d2c28f91
s4auto:OWLClass_6b9849f8_eb6a_4b0d_b135_c271d2c28f91 rdf:type owl:Class ;
                                                     rdfs:subClassOf s4auto:OWLClass_094f68a1_a622_4a62_9298_43b74210b8a4 ;
                                                     rdfs:label "Arrivals_departures_data"@es .


###  https://saref.etsi.org/saref4auto/OWLClass_71fc68af_f487_4bdf_ac37_4e79e6cd7468
s4auto:OWLClass_71fc68af_f487_4bdf_ac37_4e79e6cd7468 rdf:type owl:Class ;
                                                     rdfs:subClassOf s4auto:OWLClass_9ab327e6_b09d_41b2_93f3_a2f8970b9d72 ,
                                                                     [ rdf:type owl:Restriction ;
                                                                       owl:onProperty saref:isMeasuredIn ;
                                                                       owl:allValuesFrom s4auto:CardinalityUnit
                                                                     ] ;
                                                     rdfs:comment "Historical data" ;
                                                     rdfs:label "Number_of_passengers"@es .


###  https://saref.etsi.org/saref4auto/OWLClass_7227c333_67f8_4f2d_a0e1_208d15683bb5
s4auto:OWLClass_7227c333_67f8_4f2d_a0e1_208d15683bb5 rdf:type owl:Class ;
                                                     rdfs:subClassOf saref:UnitOfMeasure ;
                                                     rdfs:comment "To indicate the number of an entity in a fraction of time. Number per second" ;
                                                     rdfs:label "flow unit"@es .


###  https://saref.etsi.org/saref4auto/OWLClass_7507dd57_9c90_44e6_a415_770e8066fcc9
s4auto:OWLClass_7507dd57_9c90_44e6_a415_770e8066fcc9 rdf:type owl:Class ;
                                                     rdfs:subClassOf saref:Property ,
                                                                     [ rdf:type owl:Restriction ;
                                                                       owl:onProperty saref:isMeasuredIn ;
                                                                       owl:allValuesFrom s4auto:CardinalityUnit
                                                                     ] ,
                                                                     [ rdf:type owl:Restriction ;
                                                                       owl:onProperty saref:hasValue ;
                                                                       owl:someValuesFrom xsd:float
                                                                     ] ;
                                                     rdfs:label "Occupancy"@es .


###  https://saref.etsi.org/saref4auto/OWLClass_7f65788c_8f5a_4c8b_89c8_1f924c8ef511
s4auto:OWLClass_7f65788c_8f5a_4c8b_89c8_1f924c8ef511 rdf:type owl:Class ;
                                                     rdfs:subClassOf s4auto:OWLClass_d2f64388_08b5_4626_8be5_bf2614562bb8 ;
                                                     rdfs:label "Incidents_data"@es .


###  https://saref.etsi.org/saref4auto/OWLClass_836b22f0_3931_44dd_a18b_4f52f5d10379
s4auto:OWLClass_836b22f0_3931_44dd_a18b_4f52f5d10379 rdf:type owl:Class ;
                                                     rdfs:subClassOf s4auto:OWLClass_553f9409_f262_4ed9_a940_180eb68bbb2a ;
                                                     rdfs:label "Format"@es .


###  https://saref.etsi.org/saref4auto/OWLClass_8b969e76_5374_4dc6_a45d_f32e5769cafa
s4auto:OWLClass_8b969e76_5374_4dc6_a45d_f32e5769cafa rdf:type owl:Class ;
                                                     rdfs:subClassOf s4auto:OWLClass_268735bf_d97b_43a0_80f7_ead69c3861fa ;
                                                     rdfs:label "Network_data"@es .


###  https://saref.etsi.org/saref4auto/OWLClass_8cd541c9_9bb2_49a5_9820_43c0dbcf5a60
s4auto:OWLClass_8cd541c9_9bb2_49a5_9820_43c0dbcf5a60 rdf:type owl:Class ;
                                                     rdfs:subClassOf s4auto:OWLClass_836b22f0_3931_44dd_a18b_4f52f5d10379 ;
                                                     rdfs:label "GTFS"@es .


###  https://saref.etsi.org/saref4auto/OWLClass_8ef04dbb_f94e_4dae_8bf0_cb63cd807909
s4auto:OWLClass_8ef04dbb_f94e_4dae_8bf0_cb63cd807909 rdf:type owl:Class ;
                                                     rdfs:subClassOf s4auto:OWLClass_d2f64388_08b5_4626_8be5_bf2614562bb8 ,
                                                                     [ rdf:type owl:Restriction ;
                                                                       owl:onProperty saref:relatesToMeasurement ;
                                                                       owl:someValuesFrom saref:Measurement
                                                                     ] ,
                                                                     [ rdf:type owl:Restriction ;
                                                                       owl:onProperty s4auto:OWLObjectProperty_c016f3d4_1a3a_4a8b_b22d_56aaff72f689 ;
                                                                       owl:someValuesFrom saref:Property
                                                                     ] ,
                                                                     [ rdf:type owl:Restriction ;
                                                                       owl:onProperty saref:isMeasuredByDevice ;
                                                                       owl:allValuesFrom saref:Device
                                                                     ] ;
                                                     rdfs:label "Loop_detector_data"@es .


###  https://saref.etsi.org/saref4auto/OWLClass_92454d09_d714_4870_a8d4_c8c16bbc49d8
s4auto:OWLClass_92454d09_d714_4870_a8d4_c8c16bbc49d8 rdf:type owl:Class ;
                                                     rdfs:subClassOf s4auto:OWLClass_efb5f3dd_4e42_4e19_91b3_f451575038ea ,
                                                                     [ rdf:type owl:Restriction ;
                                                                       owl:onProperty saref:relatesToMeasurement ;
                                                                       owl:someValuesFrom saref:Measurement
                                                                     ] ,
                                                                     [ rdf:type owl:Restriction ;
                                                                       owl:onProperty saref:isMeasuredByDevice ;
                                                                       owl:allValuesFrom saref:Device
                                                                     ] ,
                                                                     [ rdf:type owl:Restriction ;
                                                                       owl:onProperty saref:isMeasuredIn ;
                                                                       owl:allValuesFrom s4auto:OWLClass_7227c333_67f8_4f2d_a0e1_208d15683bb5
                                                                     ] ,
                                                                     [ rdf:type owl:Restriction ;
                                                                       owl:onProperty s4auto:OWLObjectProperty_c016f3d4_1a3a_4a8b_b22d_56aaff72f689 ;
                                                                       owl:allValuesFrom s4auto:OWLClass_0f32b2d8_db89_4881_ace7_72cace8ba5de
                                                                     ] ;
                                                     rdfs:label "Pedestrian_data"@es .


###  https://saref.etsi.org/saref4auto/OWLClass_92dab589_1afc_4f99_a53c_031ddf5a1d85
s4auto:OWLClass_92dab589_1afc_4f99_a53c_031ddf5a1d85 rdf:type owl:Class ;
                                                     rdfs:subClassOf s4auto:OWLClass_efb5f3dd_4e42_4e19_91b3_f451575038ea ;
                                                     rdfs:label "Mobile_data"@es .


###  https://saref.etsi.org/saref4auto/OWLClass_9547169c_07a6_48ee_837e_27343a45ed06
s4auto:OWLClass_9547169c_07a6_48ee_837e_27343a45ed06 rdf:type owl:Class ;
                                                     rdfs:subClassOf s4auto:Vehicle ;
                                                     rdfs:label "Plane"@es .


###  https://saref.etsi.org/saref4auto/OWLClass_95be8558_d8a2_4eed_b3ac_45d78ee1d852
s4auto:OWLClass_95be8558_d8a2_4eed_b3ac_45d78ee1d852 rdf:type owl:Class ;
                                                     rdfs:subClassOf s4auto:PublicTransport ;
                                                     rdfs:label "Metro"@es .


###  https://saref.etsi.org/saref4auto/OWLClass_9ab327e6_b09d_41b2_93f3_a2f8970b9d72
s4auto:OWLClass_9ab327e6_b09d_41b2_93f3_a2f8970b9d72 rdf:type owl:Class ;
                                                     rdfs:subClassOf s4auto:OWLClass_094f68a1_a622_4a62_9298_43b74210b8a4 ;
                                                     rdfs:label "Ticketing_data"@es .


###  https://saref.etsi.org/saref4auto/OWLClass_9ac216bc_9889_42be_b873_8567be75a107
s4auto:OWLClass_9ac216bc_9889_42be_b873_8567be75a107 rdf:type owl:Class ;
                                                     rdfs:subClassOf s4auto:OWLClass_ddf85721_eecd_4df7_be3b_f513b6120358 ;
                                                     rdfs:label "Centroids"@es .


###  https://saref.etsi.org/saref4auto/OWLClass_9cf96130_d31e_4542_ab3c_d4b830de2cd6
s4auto:OWLClass_9cf96130_d31e_4542_ab3c_d4b830de2cd6 rdf:type owl:Class ;
                                                     rdfs:subClassOf geosp:Feature ,
                                                                     [ rdf:type owl:Restriction ;
                                                                       owl:onProperty s4auto:hasDescriptionName ;
                                                                       owl:someValuesFrom xsd:string
                                                                     ] ;
                                                     rdfs:label "Toll_station"@es .


###  https://saref.etsi.org/saref4auto/OWLClass_9ffbba79_32b5_41e3_9f34_6d82b4c49fe0
s4auto:OWLClass_9ffbba79_32b5_41e3_9f34_6d82b4c49fe0 rdf:type owl:Class ;
                                                     rdfs:subClassOf saref:UnitOfMeasure ;
                                                     rdfs:label "acceleration unit"@es .


###  https://saref.etsi.org/saref4auto/OWLClass_b53cfe83_28d7_4f08_a457_43738aace26a
s4auto:OWLClass_b53cfe83_28d7_4f08_a457_43738aace26a rdf:type owl:Class ;
                                                     rdfs:subClassOf s4auto:OWLClass_094f68a1_a622_4a62_9298_43b74210b8a4 ;
                                                     rdfs:label "Line_routing_data"@es .


###  https://saref.etsi.org/saref4auto/OWLClass_be6b198e_5792_4367_8dd0_e1193127a9d0
s4auto:OWLClass_be6b198e_5792_4367_8dd0_e1193127a9d0 rdf:type owl:Class ;
                                                     rdfs:subClassOf s4auto:OWLClass_f12ac0e6_d518_41b2_a737_112009debde8 ,
                                                                     [ rdf:type owl:Restriction ;
                                                                       owl:onProperty s4auto:OWLObjectProperty_e1bbccf3_d604_4a6c_a130_e2148e0787fc ;
                                                                       owl:someValuesFrom saref:Property
                                                                     ] ;
                                                     rdfs:label "Congestion_severage"@es .


###  https://saref.etsi.org/saref4auto/OWLClass_c00a4beb_8f90_4c26_bd83_6f7cfd3d5b70
s4auto:OWLClass_c00a4beb_8f90_4c26_bd83_6f7cfd3d5b70 rdf:type owl:Class ;
                                                     rdfs:subClassOf s4auto:OWLClass_ddf85721_eecd_4df7_be3b_f513b6120358 ;
                                                     rdfs:label "Connectors"@es .


###  https://saref.etsi.org/saref4auto/OWLClass_c25f950f_505d_4814_be70_0de84bc70d3c
s4auto:OWLClass_c25f950f_505d_4814_be70_0de84bc70d3c rdf:type owl:Class ;
                                                     rdfs:subClassOf s4auto:OWLClass_836b22f0_3931_44dd_a18b_4f52f5d10379 ;
                                                     rdfs:label "XML"@es .


###  https://saref.etsi.org/saref4auto/OWLClass_c4ba69f1_9f93_4d79_aff2_c354c53e0c8f
s4auto:OWLClass_c4ba69f1_9f93_4d79_aff2_c354c53e0c8f rdf:type owl:Class ;
                                                     rdfs:subClassOf saref:UnitOfMeasure ;
                                                     rdfs:comment "To indicate when each datum is caputred" ;
                                                     rdfs:label "timestamp"@es .


###  https://saref.etsi.org/saref4auto/OWLClass_c74dee04_0497_4156_bcad_06a79021d4b3
s4auto:OWLClass_c74dee04_0497_4156_bcad_06a79021d4b3 rdf:type owl:Class ;
                                                     rdfs:subClassOf s4auto:OWLClass_553f9409_f262_4ed9_a940_180eb68bbb2a ,
                                                                     [ rdf:type owl:Restriction ;
                                                                       owl:onProperty s4auto:OWLObjectProperty_10d4f71b_6da1_4eb5_840c_760db83f999d ;
                                                                       owl:someValuesFrom s4auto:OWLClass_836b22f0_3931_44dd_a18b_4f52f5d10379
                                                                     ] ;
                                                     rdfs:label "Coding_information"@es .


###  https://saref.etsi.org/saref4auto/OWLClass_ceca653f_ffb9_4523_91dd_53460e7557c0
s4auto:OWLClass_ceca653f_ffb9_4523_91dd_53460e7557c0 rdf:type owl:Class ;
                                                     rdfs:subClassOf s4auto:OWLClass_f2f0f1ca_8879_4599_8acf_34fcb5e0c2a6 ,
                                                                     [ rdf:type owl:Restriction ;
                                                                       owl:onProperty <http://www.w3.org/2003/01/geo/wgs84_pos#location> ;
                                                                       owl:allValuesFrom s4auto:Address
                                                                     ] ,
                                                                     [ rdf:type owl:Restriction ;
                                                                       owl:onProperty s4auto:OWLObjectProperty_e1bbccf3_d604_4a6c_a130_e2148e0787fc ;
                                                                       owl:allValuesFrom s4auto:OWLClass_8b969e76_5374_4dc6_a45d_f32e5769cafa
                                                                     ] ,
                                                                     [ rdf:type owl:Restriction ;
                                                                       owl:onProperty s4auto:OWLObjectProperty_e1bbccf3_d604_4a6c_a130_e2148e0787fc ;
                                                                       owl:allValuesFrom s4auto:OWLClass_b53cfe83_28d7_4f08_a457_43738aace26a
                                                                     ] ;
                                                     rdfs:label "Oxfordshire_pilot"@es .


###  https://saref.etsi.org/saref4auto/OWLClass_d2711230_22c1_49e8_8058_a44688a41a16
s4auto:OWLClass_d2711230_22c1_49e8_8058_a44688a41a16 rdf:type owl:Class ;
                                                     rdfs:subClassOf s4auto:Speed ;
                                                     rdfs:label "Average_speed"@es .


###  https://saref.etsi.org/saref4auto/OWLClass_d2f64388_08b5_4626_8be5_bf2614562bb8
s4auto:OWLClass_d2f64388_08b5_4626_8be5_bf2614562bb8 rdf:type owl:Class ;
                                                     rdfs:subClassOf s4auto:OWLClass_553f9409_f262_4ed9_a940_180eb68bbb2a ,
                                                                     [ rdf:type owl:Restriction ;
                                                                       owl:onProperty s4auto:OWLObjectProperty_10d4f71b_6da1_4eb5_840c_760db83f999d ;
                                                                       owl:someValuesFrom s4auto:OWLClass_836b22f0_3931_44dd_a18b_4f52f5d10379
                                                                     ] ,
                                                                     [ rdf:type owl:Restriction ;
                                                                       owl:onProperty s4auto:OWLObjectProperty_e1bbccf3_d604_4a6c_a130_e2148e0787fc ;
                                                                       owl:allValuesFrom s4auto:OWLClass_30dd4a6b_a368_45c4_bcb0_b2d8300ba2c1
                                                                     ] ,
                                                                     [ rdf:type owl:Restriction ;
                                                                       owl:onProperty s4auto:OWLDataProperty_60a77575_e39d_454c_96c5_66f14035eb2e ;
                                                                       owl:someValuesFrom xsd:string
                                                                     ] ,
                                                                     [ rdf:type owl:Restriction ;
                                                                       owl:onProperty s4auto:OWLDataProperty_f859b87a_028e_46d7_a87e_d75bf80fe7c7 ;
                                                                       owl:someValuesFrom xsd:string
                                                                     ] ;
                                                     rdfs:label "Traffic_data"@es .


###  https://saref.etsi.org/saref4auto/OWLClass_d53e4618_b4c4_4b81_8457_c41b82d733d4
s4auto:OWLClass_d53e4618_b4c4_4b81_8457_c41b82d733d4 rdf:type owl:Class ;
                                                     rdfs:subClassOf s4auto:OWLClass_f2f0f1ca_8879_4599_8acf_34fcb5e0c2a6 ,
                                                                     [ rdf:type owl:Restriction ;
                                                                       owl:onProperty <http://www.w3.org/2003/01/geo/wgs84_pos#location> ;
                                                                       owl:allValuesFrom s4auto:Address
                                                                     ] ,
                                                                     [ rdf:type owl:Restriction ;
                                                                       owl:onProperty s4auto:OWLObjectProperty_e1bbccf3_d604_4a6c_a130_e2148e0787fc ;
                                                                       owl:allValuesFrom s4auto:OWLClass_094f68a1_a622_4a62_9298_43b74210b8a4
                                                                     ] ,
                                                                     [ rdf:type owl:Restriction ;
                                                                       owl:onProperty s4auto:OWLObjectProperty_e1bbccf3_d604_4a6c_a130_e2148e0787fc ;
                                                                       owl:allValuesFrom s4auto:OWLClass_c74dee04_0497_4156_bcad_06a79021d4b3
                                                                     ] ,
                                                                     [ rdf:type owl:Restriction ;
                                                                       owl:onProperty s4auto:OWLObjectProperty_e1bbccf3_d604_4a6c_a130_e2148e0787fc ;
                                                                       owl:allValuesFrom s4auto:OWLClass_d2f64388_08b5_4626_8be5_bf2614562bb8
                                                                     ] ;
                                                     rdfs:label "Athens_pilot"@es .


###  https://saref.etsi.org/saref4auto/OWLClass_ddf85721_eecd_4df7_be3b_f513b6120358
s4auto:OWLClass_ddf85721_eecd_4df7_be3b_f513b6120358 rdf:type owl:Class ;
                                                     rdfs:subClassOf s4auto:OWLClass_8b969e76_5374_4dc6_a45d_f32e5769cafa ,
                                                                     [ rdf:type owl:Restriction ;
                                                                       owl:onProperty s4auto:hasAbsolutePosition ;
                                                                       owl:someValuesFrom s4auto:AbsolutePosition
                                                                     ] ;
                                                     rdfs:label "Georeferences"@es .


###  https://saref.etsi.org/saref4auto/OWLClass_eb1fda7a_fc6c_4dfb_ac2f_1ce59234bc97
s4auto:OWLClass_eb1fda7a_fc6c_4dfb_ac2f_1ce59234bc97 rdf:type owl:Class ;
                                                     rdfs:subClassOf s4auto:OWLClass_efb5f3dd_4e42_4e19_91b3_f451575038ea ,
                                                                     [ rdf:type owl:Restriction ;
                                                                       owl:onProperty saref:relatesToMeasurement ;
                                                                       owl:someValuesFrom saref:Measurement
                                                                     ] ,
                                                                     [ rdf:type owl:Restriction ;
                                                                       owl:onProperty saref:isMeasuredByDevice ;
                                                                       owl:allValuesFrom saref:Device
                                                                     ] ,
                                                                     [ rdf:type owl:Restriction ;
                                                                       owl:onProperty saref:isMeasuredIn ;
                                                                       owl:allValuesFrom s4auto:OWLClass_7227c333_67f8_4f2d_a0e1_208d15683bb5
                                                                     ] ,
                                                                     [ rdf:type owl:Restriction ;
                                                                       owl:onProperty s4auto:OWLObjectProperty_c016f3d4_1a3a_4a8b_b22d_56aaff72f689 ;
                                                                       owl:allValuesFrom s4auto:OWLClass_0f32b2d8_db89_4881_ace7_72cace8ba5de
                                                                     ] ;
                                                     rdfs:label "Bike_data"@es .


###  https://saref.etsi.org/saref4auto/OWLClass_eb247bb6_865a_4b75_9193_ba8ee763b4a2
s4auto:OWLClass_eb247bb6_865a_4b75_9193_ba8ee763b4a2 rdf:type owl:Class ;
                                                     rdfs:subClassOf s4auto:OWLClass_ddf85721_eecd_4df7_be3b_f513b6120358 ;
                                                     rdfs:label "Centroids"@es .


###  https://saref.etsi.org/saref4auto/OWLClass_efb5f3dd_4e42_4e19_91b3_f451575038ea
s4auto:OWLClass_efb5f3dd_4e42_4e19_91b3_f451575038ea rdf:type owl:Class ;
                                                     rdfs:subClassOf s4auto:OWLClass_553f9409_f262_4ed9_a940_180eb68bbb2a ,
                                                                     [ rdf:type owl:Restriction ;
                                                                       owl:onProperty s4auto:OWLObjectProperty_10d4f71b_6da1_4eb5_840c_760db83f999d ;
                                                                       owl:someValuesFrom s4auto:OWLClass_836b22f0_3931_44dd_a18b_4f52f5d10379
                                                                     ] ,
                                                                     [ rdf:type owl:Restriction ;
                                                                       owl:onProperty s4auto:OWLObjectProperty_e1bbccf3_d604_4a6c_a130_e2148e0787fc ;
                                                                       owl:allValuesFrom s4auto:OWLClass_30dd4a6b_a368_45c4_bcb0_b2d8300ba2c1
                                                                     ] ,
                                                                     [ rdf:type owl:Restriction ;
                                                                       owl:onProperty s4auto:OWLDataProperty_60a77575_e39d_454c_96c5_66f14035eb2e ;
                                                                       owl:someValuesFrom xsd:string
                                                                     ] ,
                                                                     [ rdf:type owl:Restriction ;
                                                                       owl:onProperty s4auto:OWLDataProperty_f859b87a_028e_46d7_a87e_d75bf80fe7c7 ;
                                                                       owl:someValuesFrom xsd:string
                                                                     ] ;
                                                     rdfs:label "User_data"@es .


###  https://saref.etsi.org/saref4auto/OWLClass_f12ac0e6_d518_41b2_a737_112009debde8
s4auto:OWLClass_f12ac0e6_d518_41b2_a737_112009debde8 rdf:type owl:Class ;
                                                     rdfs:subClassOf s4auto:OWLClass_d2f64388_08b5_4626_8be5_bf2614562bb8 ;
                                                     rdfs:label "Traffic_handling"@es .


###  https://saref.etsi.org/saref4auto/OWLClass_f150bbe8_b3cf_4f02_bf1d_4f0a86b669ba
s4auto:OWLClass_f150bbe8_b3cf_4f02_bf1d_4f0a86b669ba rdf:type owl:Class ;
                                                     rdfs:subClassOf saref:UnitOfMeasure ;
                                                     rdfs:label "time unit"@es .


###  https://saref.etsi.org/saref4auto/OWLClass_f2f0f1ca_8879_4599_8acf_34fcb5e0c2a6
s4auto:OWLClass_f2f0f1ca_8879_4599_8acf_34fcb5e0c2a6 rdf:type owl:Class ;
                                                     rdfs:label "Frontier"@es .


###  https://saref.etsi.org/saref4auto/OWLClass_f3514a2a_4990_46bd_b24f_ab39a8895638
s4auto:OWLClass_f3514a2a_4990_46bd_b24f_ab39a8895638 rdf:type owl:Class ;
                                                     rdfs:subClassOf s4auto:OWLClass_8b969e76_5374_4dc6_a45d_f32e5769cafa ;
                                                     rdfs:comment "GIS shapefile of study area" ;
                                                     rdfs:label "Open_street_map_data"@es .


###  https://saref.etsi.org/saref4auto/OWLClass_f4d3087f_4c57_4b40_bbf0_59a10d4f1876
s4auto:OWLClass_f4d3087f_4c57_4b40_bbf0_59a10d4f1876 rdf:type owl:Class ;
                                                     rdfs:subClassOf s4auto:OWLClass_836b22f0_3931_44dd_a18b_4f52f5d10379 ;
                                                     rdfs:label "CSV"@es .


###  https://saref.etsi.org/saref4auto/Occupied
s4auto:Occupied rdf:type owl:Class ;
                rdfs:subClassOf s4auto:ParkingSpotState ;
                rdfs:comment "A type of state for Parking Spot"@en ;
                rdfs:label "occupied"@en .


###  https://saref.etsi.org/saref4auto/P1Pedestrian
s4auto:P1Pedestrian rdf:type owl:Class ;
                    rdfs:subClassOf s4auto:VulnerableRoadUser ;
                    rdfs:comment "VRU Profile 1 users, for example: adult, child, elderly person, pram, animal, blind person guided by a dog, rider off its bike"@en ;
                    rdfs:label "P1 Pedestrian"@en .


###  https://saref.etsi.org/saref4auto/P2Bicyclist
s4auto:P2Bicyclist rdf:type owl:Class ;
                   rdfs:subClassOf s4auto:VulnerableRoadUser ;
                   rdfs:comment "VRU Profile 2 users, for example: user of bicycle, wheelchair, skater, scooter, Segway, or a mounted horse rider"@en ;
                   rdfs:label "P2 Bicyclist"@en .


###  https://saref.etsi.org/saref4auto/P3Motorcyclist
s4auto:P3Motorcyclist rdf:type owl:Class ;
                      rdfs:subClassOf s4auto:VulnerableRoadUser ;
                      rdfs:comment "VRU Profile 3 users are Motorcyclists, which are equipped with engines that allow them to move on the road. It includes users (driver and passengers, e.g. children and animals) of Powered Two Wheelers (PTW) such as mopeds (motorized scooters), motorcycles or side-cars."@en ;
                      rdfs:label "P3 Motorcyclist"@en .


###  https://saref.etsi.org/saref4auto/P4Animal
s4auto:P4Animal rdf:type owl:Class ;
                rdfs:subClassOf s4auto:VulnerableRoadUser ;
                rdfs:comment "VRU Profile 4 animals presenting a safety risk to other road users, for example : dogs, wild animals, horses, cows, sheep, kangaroos, etc."@en ;
                rdfs:label "P4 Animal"@en .


###  https://saref.etsi.org/saref4auto/Parked
s4auto:Parked rdf:type owl:Class ;
              rdfs:subClassOf s4auto:ParkingVehicleState ;
              rdfs:comment "A type of state for Parking Vehicle"@en ;
              rdfs:label "parked"@en .


###  https://saref.etsi.org/saref4auto/Parking
s4auto:Parking rdf:type owl:Class ;
               rdfs:subClassOf s4auto:ParkingVehicleState ;
               rdfs:comment "A type of state for Parking Vehicle"@en ;
               rdfs:label "parking"@en .


###  https://saref.etsi.org/saref4auto/ParkingSpot
s4auto:ParkingSpot rdf:type owl:Class ;
                   rdfs:subClassOf geosp:Feature ,
                                   [ rdf:type owl:Restriction ;
                                     owl:onProperty geosp:hasGeometry ;
                                     owl:someValuesFrom s4auto:ParkingSpotPoint
                                   ] ,
                                   [ rdf:type owl:Restriction ;
                                     owl:onProperty s4auto:hasHeight ;
                                     owl:someValuesFrom s4auto:Height
                                   ] ,
                                   [ rdf:type owl:Restriction ;
                                     owl:onProperty s4auto:hasIdentifier ;
                                     owl:someValuesFrom s4auto:Identifier
                                   ] ,
                                   [ rdf:type owl:Restriction ;
                                     owl:onProperty s4auto:hasLength ;
                                     owl:someValuesFrom s4auto:Length
                                   ] ,
                                   [ rdf:type owl:Restriction ;
                                     owl:onProperty s4auto:hasOpeningTimeAvailability ;
                                     owl:someValuesFrom time:TemporalEntity
                                   ] ,
                                   [ rdf:type owl:Restriction ;
                                     owl:onProperty s4auto:hasWidth ;
                                     owl:someValuesFrom s4auto:Width
                                   ] ,
                                   [ rdf:type owl:Restriction ;
                                     owl:onProperty s4auto:hasParkingSpotState ;
                                     owl:maxQualifiedCardinality "1"^^xsd:nonNegativeInteger ;
                                     owl:onClass s4auto:ParkingSpotState
                                   ] ,
                                   [ rdf:type owl:Restriction ;
                                     owl:onProperty s4auto:hasDescriptionName ;
                                     owl:someValuesFrom xsd:string
                                   ] ;
                   rdfs:comment "A location that is designated for parking. A parking spot has a geometry defining the parking area boundaries and its centre point"@en ;
                   rdfs:label "ParkingSpot"@en .


###  https://saref.etsi.org/saref4auto/ParkingSpotPoint
s4auto:ParkingSpotPoint rdf:type owl:Class ;
                        rdfs:subClassOf s4auto:Point ;
                        rdfs:comment "the position of aparking spot (its centre point) in terms of lat, long and alt"@en ;
                        rdfs:label "ParkingSpotPoint"@en .


###  https://saref.etsi.org/saref4auto/ParkingSpotState
s4auto:ParkingSpotState rdf:type owl:Class ;
                        rdfs:subClassOf s4auto:State ;
                        rdfs:comment "A parking spot has a state. Possible values for parking spot state are Free, occupied, reserved, closed, charging"@en ;
                        rdfs:label "ParkingSpotState"@en .


###  https://saref.etsi.org/saref4auto/ParkingVehicleState
s4auto:ParkingVehicleState rdf:type owl:Class ;
                           rdfs:subClassOf s4auto:State ;
                           rdfs:comment "A vehicle can be found at different states (or parking phases) during parking . Possible values for parking state (or parking phase) of a vehicle are: At drop-off spot, at pick-up spot, driving to parking spot, driving to pick up spot, parking, parked, charging."@en ;
                           rdfs:label "ParkingVehicleState"@en .


###  https://saref.etsi.org/saref4auto/PassengerCar
s4auto:PassengerCar rdf:type owl:Class ;
                    rdfs:subClassOf s4auto:Car ;
                    rdfs:comment "A type of car"@en ;
                    rdfs:label "PassengerCar"@en .


###  https://saref.etsi.org/saref4auto/PerceptionState
s4auto:PerceptionState rdf:type owl:Class ;
                       rdfs:subClassOf s4auto:State ;
                       rdfs:comment "A state of the vehicle related to its environment"@en ;
                       rdfs:label "perception state"@en .


###  https://saref.etsi.org/saref4auto/PersonalDevice
s4auto:PersonalDevice rdf:type owl:Class ;
                      rdfs:subClassOf saref:Device ,
                                      s4auto:AutomotiveObject ;
                      rdfs:comment "A personal device is a nomadic device used by a pedestrian or the rider of a two-wheeler. A personal device in modelled as a different type of automotive object, as it normally does not have access to the vehicle CAN bus."@en ;
                      rdfs:label "PersonalDevice"@en .


###  https://saref.etsi.org/saref4auto/Platoon
s4auto:Platoon rdf:type owl:Class ;
               rdfs:subClassOf [ rdf:type owl:Restriction ;
                                 owl:onProperty s4auto:hasDestinationEndPoint ;
                                 owl:someValuesFrom s4auto:EndPoint
                               ] ,
                               [ rdf:type owl:Restriction ;
                                 owl:onProperty s4auto:hasIdentifier ;
                                 owl:someValuesFrom s4auto:Identifier
                               ] ,
                               [ rdf:type owl:Restriction ;
                                 owl:onProperty s4auto:hasLength ;
                                 owl:someValuesFrom s4auto:Length
                               ] ,
                               [ rdf:type owl:Restriction ;
                                 owl:onProperty s4auto:hasPlatoonMember ;
                                 owl:someValuesFrom s4auto:Vehicle
                               ] ,
                               [ rdf:type owl:Restriction ;
                                 owl:onProperty s4auto:hasPlatoonState ;
                                 owl:someValuesFrom s4auto:PlatoonState
                               ] ,
                               [ rdf:type owl:Restriction ;
                                 owl:onProperty s4auto:hasRoute ;
                                 owl:someValuesFrom s4auto:Route
                               ] ,
                               [ rdf:type owl:Restriction ;
                                 owl:onProperty s4auto:hasSize ;
                                 owl:someValuesFrom s4auto:Size
                               ] ,
                               [ rdf:type owl:Restriction ;
                                 owl:onProperty s4auto:hasMaxSize ;
                                 owl:someValuesFrom xsd:int
                               ] ;
               rdfs:comment "A group of vehicles automatically following each other at a relatively close distance" ;
               rdfs:label "Platoon"@en .


###  https://saref.etsi.org/saref4auto/PlatoonAutomationLevel
s4auto:PlatoonAutomationLevel rdf:type owl:Class ;
                              rdfs:subClassOf s4auto:AutomationLevel ;
                              rdfs:comment "A level of automation is defined for a vehicle that it is platooning. For example, in the ENSEMBLE project  there are three levels of platoon automation defined: Level A, Level B, Level C. Level C represents the highest level of automation for platooning in terms of longitudinal and lateral control, shortest time gap supported, wider range of situations handled and support for merging of entire platoons."@en ;
                              rdfs:label "PlatoonAutomationLevel"@en .


###  https://saref.etsi.org/saref4auto/PlatoonPosition
s4auto:PlatoonPosition rdf:type owl:Class ;
                       rdfs:subClassOf s4auto:Position ,
                                       [ rdf:type owl:Restriction ;
                                         owl:onProperty s4auto:hasPlatoonIndex ;
                                         owl:someValuesFrom xsd:int
                                       ] ;
                       rdfs:comment "A vehicle member of a platoon has a platoon position that is defined as the index of the vehicle in the platoon starting from zero (leader) up to N (trailing vehicle)."@en ;
                       rdfs:label "PlatoonPosition"@en .


###  https://saref.etsi.org/saref4auto/PlatoonRole
s4auto:PlatoonRole rdf:type owl:Class ;
                   rdfs:subClassOf s4auto:Role ;
                   rdfs:comment "In platoon a vehicle can assume roles such as: unknown, leader, follower, ready-for-leading, trailing, etc."@en ;
                   rdfs:label "PlatoonRole"@en .


###  https://saref.etsi.org/saref4auto/PlatoonState
s4auto:PlatoonState rdf:type owl:Class ;
                    rdfs:subClassOf s4auto:State ;
                    rdfs:comment "The state of a platoon. Examples of states for a platoon are: unknown, standalone, assembling, platooning, disengaging, etc."@en ;
                    rdfs:label "PlatoonState"@en .


###  https://saref.etsi.org/saref4auto/PlatoonVehicleState
s4auto:PlatoonVehicleState rdf:type owl:Class ;
                           rdfs:subClassOf s4auto:State ;
                           rdfs:comment "Examples of states for a vehicle in a platoon are: unknown, standalone, engaging, platooning, disengaging, searching, forming."@en ;
                           rdfs:label "PlatoonVehicleState"@en .


###  https://saref.etsi.org/saref4auto/Platooning
s4auto:Platooning rdf:type owl:Class ;
                  rdfs:subClassOf s4auto:PlatoonState ,
                                  s4auto:PlatoonVehicleState ;
                  rdfs:comment "A type of state for Platoon or for a Vehicle in a Platoon"@en ;
                  rdfs:label "platooning"@en .


###  https://saref.etsi.org/saref4auto/Point
s4auto:Point rdf:type owl:Class ;
             rdfs:subClassOf geosp:Geometry ,
                             <http://www.w3.org/2003/01/geo/wgs84_pos#Point> ;
             rdfs:comment "A geo point in SAREF4AUTO"@en ;
             rdfs:label "Point"@en .


###  https://saref.etsi.org/saref4auto/Position
s4auto:Position rdf:type owl:Class ;
                rdfs:subClassOf [ rdf:type owl:Restriction ;
                                  owl:onProperty s4auto:hasConfidence ;
                                  owl:someValuesFrom s4auto:Confidence
                                ] ;
                rdfs:comment "The position of an entity in the automotive domain"@en ;
                rdfs:label "Position"@en .


###  https://saref.etsi.org/saref4auto/PositionConfidenceEllipse
s4auto:PositionConfidenceEllipse rdf:type owl:Class ;
                                 rdfs:subClassOf s4auto:Confidence ;
                                 rdfs:comment "A type of confidence that represents horizontal position accuracy in a shape of ellipse with a predefined confidence level (e.g. 95 %). The centre of the ellipse shape corresponds to the reference position point for which the position accuracy is evaluated."@en ;
                                 rdfs:label "PositionConfidenceEllipse"@en .


###  https://saref.etsi.org/saref4auto/PublicTransport
s4auto:PublicTransport rdf:type owl:Class ;
                       rdfs:subClassOf s4auto:Vehicle .


###  https://saref.etsi.org/saref4auto/RegularParkingSpot
s4auto:RegularParkingSpot rdf:type owl:Class ;
                          rdfs:subClassOf s4auto:ParkingSpot ;
                          rdfs:comment "A type pf parking spot"@en ;
                          rdfs:label "RegularParkingSpot"@en .


###  https://saref.etsi.org/saref4auto/RelativePosition
s4auto:RelativePosition rdf:type owl:Class ;
                        rdfs:subClassOf s4auto:Position ,
                                        [ rdf:type owl:Restriction ;
                                          owl:onProperty s4auto:hasCoordinateX ;
                                          owl:someValuesFrom xsd:float
                                        ] ,
                                        [ rdf:type owl:Restriction ;
                                          owl:onProperty s4auto:hasCoordinateY ;
                                          owl:someValuesFrom xsd:float
                                        ] ,
                                        [ rdf:type owl:Restriction ;
                                          owl:onProperty s4auto:hasCoordinateZ ;
                                          owl:someValuesFrom xsd:float
                                        ] ;
                        rdfs:comment "It represents the relative position of a vehicle (e.g., a car is x,y,z in front of another car)"@en ;
                        rdfs:label "RelativePosition"@en .


###  https://saref.etsi.org/saref4auto/RelativeSpeed
s4auto:RelativeSpeed rdf:type owl:Class ;
                     rdfs:subClassOf s4auto:Speed ;
                     rdfs:comment "A type of speed"@en ;
                     rdfs:label "RelativeSpeed"@en .


###  https://saref.etsi.org/saref4auto/RendezvousLocation
s4auto:RendezvousLocation rdf:type owl:Class ;
                          rdfs:subClassOf s4auto:Point ;
                          rdfs:comment "It is the estimated location where the vehicle member joins the platoon. It is expressed in global coordinates (lat, long, alt), e.g. according to WGS 84."@en ;
                          rdfs:label "RendezvousLocation"@en .


###  https://saref.etsi.org/saref4auto/Reserved
s4auto:Reserved rdf:type owl:Class ;
                rdfs:subClassOf s4auto:ParkingSpotState ;
                rdfs:comment "A type of state for Parking Spot"@en ;
                rdfs:label "reserved"@en .


###  https://saref.etsi.org/saref4auto/RoadEntity
s4auto:RoadEntity rdf:type owl:Class ;
                  rdfs:subClassOf saref:FeatureOfInterest ,
                                  [ rdf:type owl:Restriction ;
                                    owl:onProperty s4auto:consistsOfEquipment ;
                                    owl:someValuesFrom s4auto:RoadSideEquipment
                                  ] ,
                                  [ rdf:type owl:Restriction ;
                                    owl:onProperty s4auto:consistsOfEvent ;
                                    owl:someValuesFrom s4auto:NotifiedEvent
                                  ] ,
                                  [ rdf:type owl:Restriction ;
                                    owl:onProperty s4auto:consistsOfObject ;
                                    owl:someValuesFrom s4auto:CriticalObject
                                  ] ,
                                  [ rdf:type owl:Restriction ;
                                    owl:onProperty s4auto:consistsOfUser ;
                                    owl:someValuesFrom s4auto:VulnerableRoadUser
                                  ] ,
                                  [ rdf:type owl:Restriction ;
                                    owl:onProperty s4auto:hasAbsolutePosition ;
                                    owl:someValuesFrom s4auto:AbsolutePosition
                                  ] ,
                                  [ rdf:type owl:Restriction ;
                                    owl:onProperty s4auto:hasHeight ;
                                    owl:someValuesFrom s4auto:Height
                                  ] ,
                                  [ rdf:type owl:Restriction ;
                                    owl:onProperty s4auto:hasLength ;
                                    owl:someValuesFrom s4auto:Length
                                  ] ,
                                  [ rdf:type owl:Restriction ;
                                    owl:onProperty s4auto:hasMovement ;
                                    owl:someValuesFrom s4auto:Movement
                                  ] ,
                                  [ rdf:type owl:Restriction ;
                                    owl:onProperty s4auto:hasRelativePosition ;
                                    owl:someValuesFrom s4auto:RelativePosition
                                  ] ,
                                  [ rdf:type owl:Restriction ;
                                    owl:onProperty s4auto:hasShape ;
                                    owl:someValuesFrom s4auto:Shape
                                  ] ,
                                  [ rdf:type owl:Restriction ;
                                    owl:onProperty s4auto:hasWidth ;
                                    owl:someValuesFrom s4auto:Width
                                  ] ;
                  rdfs:comment "An entity present on the road in the neighbouring area of a vehicle"@en ;
                  rdfs:label "RoadEntity"@en .


###  https://saref.etsi.org/saref4auto/RoadObject
s4auto:RoadObject rdf:type owl:Class ;
                  rdfs:subClassOf saref:FeatureOfInterest ;
                  rdfs:comment "Road side sensors measure properties (such as speed, position, dimension, direction, etc.) of road objects. Types of relevant road objects are Pedestrian, vehicles, obstacles, traffic signs, etc."@en ;
                  rdfs:label "RoadObject"@en .


###  https://saref.etsi.org/saref4auto/RoadSideActuator
s4auto:RoadSideActuator rdf:type owl:Class ;
                        rdfs:subClassOf saref:Actuator ,
                                        [ rdf:type owl:Restriction ;
                                          owl:onProperty s4auto:usesMeasurement ;
                                          owl:someValuesFrom saref:Measurement
                                        ] ;
                        rdfs:comment "Devices deployed along the road that produce signals based on road side sensor data measurements. Types of road side actuators that are relevant are devices such as traffic light controllers changing from red to green based on detected vehicles."@en ;
                        rdfs:label """RoadSideActuator
"""@en .


###  https://saref.etsi.org/saref4auto/RoadSideEquipment
s4auto:RoadSideEquipment rdf:type owl:Class ;
                         rdfs:subClassOf s4auto:AutomotiveObject ;
                         rdfs:comment "A road side equipment can be either a simple data relay between vehicles and infrastructure or between the vehicles themselves, or it can run applications. It is usually high mounted in existing equipment, such as a street light, city traffic light, VMS or highway sign, or has its own pole."@en ;
                         rdfs:label "RoadSideEquipment"@en .


###  https://saref.etsi.org/saref4auto/RoadSideSensor
s4auto:RoadSideSensor rdf:type owl:Class ;
                      rdfs:subClassOf saref:Sensor ,
                                      [ rdf:type owl:Restriction ;
                                        owl:onProperty saref:measuresProperty ;
                                        owl:someValuesFrom s4auto:Heading
                                      ] ,
                                      [ rdf:type owl:Restriction ;
                                        owl:onProperty saref:measuresProperty ;
                                        owl:someValuesFrom s4auto:Height
                                      ] ,
                                      [ rdf:type owl:Restriction ;
                                        owl:onProperty saref:measuresProperty ;
                                        owl:someValuesFrom s4auto:Length
                                      ] ,
                                      [ rdf:type owl:Restriction ;
                                        owl:onProperty saref:measuresProperty ;
                                        owl:someValuesFrom s4auto:OWLClass_0f32b2d8_db89_4881_ace7_72cace8ba5de
                                      ] ,
                                      [ rdf:type owl:Restriction ;
                                        owl:onProperty saref:measuresProperty ;
                                        owl:someValuesFrom s4auto:OWLClass_7507dd57_9c90_44e6_a415_770e8066fcc9
                                      ] ,
                                      [ rdf:type owl:Restriction ;
                                        owl:onProperty saref:measuresProperty ;
                                        owl:someValuesFrom s4auto:Speed
                                      ] ,
                                      [ rdf:type owl:Restriction ;
                                        owl:onProperty saref:measuresProperty ;
                                        owl:someValuesFrom s4auto:Width
                                      ] ,
                                      [ rdf:type owl:Restriction ;
                                        owl:onProperty s4auto:detectsPosition ;
                                        owl:someValuesFrom s4auto:AbsolutePosition
                                      ] ,
                                      [ rdf:type owl:Restriction ;
                                        owl:onProperty s4auto:detectsPosition ;
                                        owl:someValuesFrom s4auto:RelativePosition
                                      ] ;
                      rdfs:comment "Sensors such as cameras, radars that are deployed along the road (e.g. at intersections and at poles along a highway). Road side sensors perform measurements, such as speed, position (relative or absolute), dimension, direction, etc. of road objects."@en ;
                      rdfs:label "RoadSideSensor"@en .


###  https://saref.etsi.org/saref4auto/RoadTopologyPosition
s4auto:RoadTopologyPosition rdf:type owl:Class ;
                            rdfs:subClassOf s4auto:Position ;
                            rdfs:comment "Position with respect to road topology (e.g. road, segment or lane) and lane characteristics (highway lane, road lane, bicycle lane, pavement, off-road)."@en ;
                            rdfs:label "Road Topology Position"@en .


###  https://saref.etsi.org/saref4auto/Role
s4auto:Role rdf:type owl:Class ;
            rdfs:comment "The role that can be assumed by a vehicle or a platoon"@en ;
            rdfs:label "Role"@en .


###  https://saref.etsi.org/saref4auto/Route
s4auto:Route rdf:type owl:Class ;
             rdfs:subClassOf [ rdf:type owl:Restriction ;
                               owl:onProperty s4auto:hasDestinationEndPoint ;
                               owl:someValuesFrom s4auto:EndPoint
                             ] ,
                             [ rdf:type owl:Restriction ;
                               owl:onProperty s4auto:hasOrigin ;
                               owl:someValuesFrom s4auto:StartPoint
                             ] ,
                             [ rdf:type owl:Restriction ;
                               owl:onProperty s4auto:isCollectionOf ;
                               owl:someValuesFrom s4auto:RoutePoint
                             ] ;
             rdfs:comment "The route of a vehicle or of a platoon. The route of a platoon is defined as the route of the current vehicle leader in the platoon that other follower vehicles (partially) share"@en ;
             rdfs:label "Route"@en .


###  https://saref.etsi.org/saref4auto/RoutePoint
s4auto:RoutePoint rdf:type owl:Class ;
                  rdfs:subClassOf s4auto:Point ;
                  rdfs:comment "The intermediate points of a route"@en ;
                  rdfs:label "RoutePoint"@en .


###  https://saref.etsi.org/saref4auto/Searching
s4auto:Searching rdf:type owl:Class ;
                 rdfs:subClassOf s4auto:PlatoonVehicleState ;
                 rdfs:comment "A type of state for a Vehicle in a Platoon"@en ;
                 rdfs:label "Searching"@en .


###  https://saref.etsi.org/saref4auto/Shape
s4auto:Shape rdf:type owl:Class ;
             rdfs:subClassOf saref:Property ;
             rdfs:comment "A Property of interest for the automotive domain. It defines the overall shape of an entity: i.e., Sphere, Torus, Cylinder, Cone, Ellipsoid, Cube, Cuboid, Pyramid, Prism, Multiple shapes"@en ;
             rdfs:label "Shape"@en .


###  https://saref.etsi.org/saref4auto/Size
s4auto:Size rdf:type owl:Class ;
            rdfs:subClassOf <http://www.w3.org/2003/01/geo/wgs84_pos#Point> ;
            rdfs:comment "A Property of interest for the automotive domain. A platoon has a size. Tis size is defined as 1) the total number of vehicles currently in the platoon; or 2) Length of the platoon (sum of all vehicles' length + inter-vehicle distance)"@en ;
            rdfs:label "Size"@en .


###  https://saref.etsi.org/saref4auto/SmallObject
s4auto:SmallObject rdf:type owl:Class ;
                   rdfs:subClassOf s4auto:CriticalObject ;
                   rdfs:comment "A type of Critical Object"@en ;
                   rdfs:label "Small Object"@en .


###  https://saref.etsi.org/saref4auto/SpecialPermitParkingSpot
s4auto:SpecialPermitParkingSpot rdf:type owl:Class ;
                                rdfs:subClassOf s4auto:ParkingSpot ;
                                rdfs:comment "A type pf parking spot. Parking spot reserved for special permits (authorities, disabled, blue Zone, resident ...)"@en ;
                                rdfs:label "SpecialPermitParkingSpot"@en .


###  https://saref.etsi.org/saref4auto/Speed
s4auto:Speed rdf:type owl:Class ;
             rdfs:subClassOf saref:Property ,
                             [ rdf:type owl:Restriction ;
                               owl:onProperty saref:isMeasuredIn ;
                               owl:allValuesFrom s4auto:SpeedUnit
                             ] ,
                             [ rdf:type owl:Restriction ;
                               owl:onProperty saref:hasValue ;
                               owl:someValuesFrom xsd:float
                             ] ;
             rdfs:comment "A Property of interest for the automotive domain"@en ;
             rdfs:label "Speed"@en .


###  https://saref.etsi.org/saref4auto/SpeedConfidence
s4auto:SpeedConfidence rdf:type owl:Class ;
                       rdfs:subClassOf s4auto:Confidence ,
                                       [ rdf:type owl:Restriction ;
                                         owl:onProperty s4auto:hasConfidenceValue ;
                                         owl:someValuesFrom xsd:int
                                       ] ;
                       rdfs:comment "A type of confidence for speed measurements that represents absolute accuracy of a speed value in cm/s"@en ;
                       rdfs:label "SpeedConfidence"@en .


###  https://saref.etsi.org/saref4auto/SpeedUnit
s4auto:SpeedUnit rdf:type owl:Class ;
                 rdfs:subClassOf saref:UnitOfMeasure ;
                 rdfs:comment "unit of measure of speed"@en ;
                 rdfs:label "speed unit"@en .


###  https://saref.etsi.org/saref4auto/Standalone
s4auto:Standalone rdf:type owl:Class ;
                  rdfs:subClassOf s4auto:PlatoonState ,
                                  s4auto:PlatoonVehicleState ;
                  rdfs:comment "A type of state for Platoon or for a Vehicle in a Platoon"@en ;
                  rdfs:label "standalone"@en .


###  https://saref.etsi.org/saref4auto/StartPoint
s4auto:StartPoint rdf:type owl:Class ;
                  rdfs:subClassOf s4auto:Point ;
                  rdfs:comment "The origin of a route"@en ;
                  rdfs:label "StartPoint"@en .


###  https://saref.etsi.org/saref4auto/State
s4auto:State rdf:type owl:Class ;
             rdfs:subClassOf saref:State ,
                             [ rdf:type owl:Restriction ;
                               owl:onProperty saref:hasTimestamp ;
                               owl:someValuesFrom xsd:dateTime
                             ] ;
             rdfs:comment "A class dedicated to describe the relevant states in the automotive domain"@en ;
             rdfs:label "State"@en .


###  https://saref.etsi.org/saref4auto/StationID
s4auto:StationID rdf:type owl:Class ;
                 rdfs:subClassOf s4auto:Identifier ;
                 rdfs:comment "A type of identifier for vehicles and platoons, as defined in ETSI TS 102 894-2."@en ;
                 rdfs:label "StationID"@en .


###  https://saref.etsi.org/saref4auto/TrafficLightController
s4auto:TrafficLightController rdf:type owl:Class ;
                              rdfs:subClassOf s4auto:RoadSideActuator ;
                              rdfs:comment "A device that automatically operates coloured lights, typically red, amber, and green, for controlling traffic at road junctions, pedestrian crossings, and roundabouts."@en ;
                              rdfs:label "TrafficLight"@en .


###  https://saref.etsi.org/saref4auto/TrafficManagementCentre
s4auto:TrafficManagementCentre rdf:type owl:Class ;
                               rdfs:subClassOf s4auto:AutomotiveObject ;
                               rdfs:comment "A traffic centre provides services to road users: exploiting data for road traffic management, providing information about mobility zones, operational management of the road infrastructure, etc."@en ;
                               rdfs:label "TrafficManagementCentre"@en .


###  https://saref.etsi.org/saref4auto/Tram
s4auto:Tram rdf:type owl:Class ;
            rdfs:subClassOf s4auto:PublicTransport ;
            rdfs:comment "A type of public transport"@en ;
            rdfs:label "tram"@en .


###  https://saref.etsi.org/saref4auto/Truck
s4auto:Truck rdf:type owl:Class ;
             rdfs:subClassOf s4auto:Vehicle ;
             rdfs:comment "A type of vehicle. Example of trucks are heavy trucks or light trucks."@en ;
             rdfs:label "Truck"@en .


###  https://saref.etsi.org/saref4auto/TwoWheeler
s4auto:TwoWheeler rdf:type owl:Class ;
                  rdfs:subClassOf s4auto:Vehicle ;
                  rdfs:comment "A type of vehicle. This class involves all sorts of two wheelers, from motorcycles to bicycles and (e-)scooters."@en ;
                  rdfs:label "TwoWheeler"@en .


###  https://saref.etsi.org/saref4auto/UUID
s4auto:UUID rdf:type owl:Class ;
            rdfs:subClassOf s4auto:Identifier ;
            rdfs:comment "A universally unique identifier (UUID) is a 128-bit number used to identify items and is also known as: globally unique identifier (GUID). In its canonical textual representation, the sixteen octets of a UUID are represented as 32 hexadecimal (base 16) digits, displayed in five groups separated by hyphens, in the form 8-4-4-4-12 for a total of 36 characters (32 alphanumeric characters and four hyphens). UUID are documented in ISO/IEC 11578:1996 \"Information technology – Open Systems Interconnection – Remote Procedure Call (RPC)\" and in ITU-T Rec. X.667 ISO/IEC 9834-8:2005."@en ;
            rdfs:label "UUID"@en .


###  https://saref.etsi.org/saref4auto/Unknown
s4auto:Unknown rdf:type owl:Class ;
               rdfs:subClassOf s4auto:PlatoonState ,
                               s4auto:PlatoonVehicleState .


###  https://saref.etsi.org/saref4auto/Vehicle
s4auto:Vehicle rdf:type owl:Class ;
               rdfs:subClassOf saref:FeatureOfInterest ,
                               s4auto:AutomotiveObject ,
                               s4syst:System ,
                               [ rdf:type owl:Restriction ;
                                 owl:onProperty s4auto:hasAbsolutePosition ;
                                 owl:someValuesFrom s4auto:AbsolutePosition
                               ] ,
                               [ rdf:type owl:Restriction ;
                                 owl:onProperty s4auto:hasAutomationLevel ;
                                 owl:someValuesFrom s4auto:AutomationLevel
                               ] ,
                               [ rdf:type owl:Restriction ;
                                 owl:onProperty s4auto:hasBrakeCapacity ;
                                 owl:someValuesFrom s4auto:BrakeCapacity
                               ] ,
                               [ rdf:type owl:Restriction ;
                                 owl:onProperty s4auto:hasDestinationAddress ;
                                 owl:someValuesFrom s4auto:Address
                               ] ,
                               [ rdf:type owl:Restriction ;
                                 owl:onProperty s4auto:hasDestinationEndPoint ;
                                 owl:someValuesFrom s4auto:EndPoint
                               ] ,
                               [ rdf:type owl:Restriction ;
                                 owl:onProperty s4auto:hasEnvironment ;
                                 owl:someValuesFrom s4auto:VehicleEnvironment
                               ] ,
                               [ rdf:type owl:Restriction ;
                                 owl:onProperty s4auto:hasEstimatedRendezvousLocation ;
                                 owl:someValuesFrom s4auto:RendezvousLocation
                               ] ,
                               [ rdf:type owl:Restriction ;
                                 owl:onProperty s4auto:hasHeight ;
                                 owl:someValuesFrom s4auto:Height
                               ] ,
                               [ rdf:type owl:Restriction ;
                                 owl:onProperty s4auto:hasIdentifier ;
                                 owl:someValuesFrom s4auto:Identifier
                               ] ,
                               [ rdf:type owl:Restriction ;
                                 owl:onProperty s4auto:hasLength ;
                                 owl:someValuesFrom s4auto:Length
                               ] ,
                               [ rdf:type owl:Restriction ;
                                 owl:onProperty s4auto:hasParkingVehicleState ;
                                 owl:someValuesFrom s4auto:PlatoonVehicleState
                               ] ,
                               [ rdf:type owl:Restriction ;
                                 owl:onProperty s4auto:hasPlatoonPosition ;
                                 owl:someValuesFrom s4auto:PlatoonPosition
                               ] ,
                               [ rdf:type owl:Restriction ;
                                 owl:onProperty s4auto:hasPlatoonRole ;
                                 owl:someValuesFrom s4auto:PlatoonRole
                               ] ,
                               [ rdf:type owl:Restriction ;
                                 owl:onProperty s4auto:hasPlatoonVehicleState ;
                                 owl:someValuesFrom s4auto:PlatoonVehicleState
                               ] ,
                               [ rdf:type owl:Restriction ;
                                 owl:onProperty s4auto:hasRelativePosition ;
                                 owl:someValuesFrom s4auto:RelativePosition
                               ] ,
                               [ rdf:type owl:Restriction ;
                                 owl:onProperty s4auto:hasRoadTopologyPosition ;
                                 owl:someValuesFrom s4auto:RoadTopologyPosition
                               ] ,
                               [ rdf:type owl:Restriction ;
                                 owl:onProperty s4auto:hasRoute ;
                                 owl:someValuesFrom s4auto:Route
                               ] ,
                               [ rdf:type owl:Restriction ;
                                 owl:onProperty s4auto:hasVehicleRole ;
                                 owl:someValuesFrom s4auto:VehicleRole
                               ] ,
                               [ rdf:type owl:Restriction ;
                                 owl:onProperty s4auto:hasWidth ;
                                 owl:someValuesFrom s4auto:Width
                               ] ,
                               [ rdf:type owl:Restriction ;
                                 owl:onProperty s4auto:isMemberOfPlatoon ;
                                 owl:someValuesFrom s4auto:Platoon
                               ] ,
                               [ rdf:type owl:Restriction ;
                                 owl:onProperty s4auto:isMemberOfVehicleEnvironment ;
                                 owl:someValuesFrom s4auto:VehicleEnvironment
                               ] ,
                               [ rdf:type owl:Restriction ;
                                 owl:onProperty s4syst:hasSubSystem ;
                                 owl:someValuesFrom s4auto:ElectronicControlUnit
                               ] ,
                               [ rdf:type owl:Restriction ;
                                 owl:onProperty s4auto:hasEstimatedJoiningTime ;
                                 owl:someValuesFrom xsd:dateTime
                               ] ;
               rdfs:comment "A vehicle is the main object of interest in the automotive domain. Example of types of vehicles are car, truck, public transport and two-wheeler. See ETSI TS 102 894-2 spec for full list of vehicles, which are type of \"stations\". See also the SENSORIS data model for possible type of vehicles. The main IoT device considered in the vehicle is the ECU (part of the vehicle on board equipment, or OBE), see s4auto:ElectronicControlUnit class."@en ;
               rdfs:label "Vehicle"@en .


###  https://saref.etsi.org/saref4auto/VehicleAutomationLevel
s4auto:VehicleAutomationLevel rdf:type owl:Class ;
                              rdfs:subClassOf s4auto:AutomationLevel ;
                              rdfs:comment """According to SAE J3016, there are five levels of automation for a vehicle:
- Level 0: No Driving Automation.
- Level 1: Driver assistance.
- Level 2: Partial driving automation.
- Level 3: Conditional driving automation.
- Level 4: High driving automation.
- Level 5: Full Driving automation."""@en ;
                              rdfs:label "VehicleAutomationLevel"@en .


###  https://saref.etsi.org/saref4auto/VehicleEnvironment
s4auto:VehicleEnvironment rdf:type owl:Class ;
                          rdfs:subClassOf [ rdf:type owl:Restriction ;
                                            owl:onProperty s4auto:consistsOfEntity ;
                                            owl:someValuesFrom s4auto:RoadEntity
                                          ] ,
                                          [ rdf:type owl:Restriction ;
                                            owl:onProperty s4auto:consistsOfVehicle ;
                                            owl:someValuesFrom s4auto:Vehicle
                                          ] ;
                          rdfs:comment "The vehicle environment is made of entities which are present on the road in the area around the vehicle"@en ;
                          rdfs:label "VehicleEnvironment"@en .


###  https://saref.etsi.org/saref4auto/VehicleRole
s4auto:VehicleRole rdf:type owl:Class ;
                   rdfs:subClassOf s4auto:Role ;
                   rdfs:comment "The role the vehicle plays in traffic. If not specified, it is assumed that it takes a default value. Otherwise, possible values to be specified are: publicTransport, specialTransport, dangerousGoods, roadWork, rescue, emergency, safetyCar, agriculture, commercial, military, roadOperator, taxi."@en ;
                   rdfs:label "VehicleRole"@en .


###  https://saref.etsi.org/saref4auto/VulnerableRoadUser
s4auto:VulnerableRoadUser rdf:type owl:Class ;
                          rdfs:subClassOf owl:Thing ,
                                          [ rdf:type owl:Restriction ;
                                            owl:onProperty s4auto:hasHeight ;
                                            owl:someValuesFrom s4auto:Height
                                          ] ,
                                          [ rdf:type owl:Restriction ;
                                            owl:onProperty s4auto:hasLength ;
                                            owl:someValuesFrom s4auto:Length
                                          ] ,
                                          [ rdf:type owl:Restriction ;
                                            owl:onProperty s4auto:hasMovement ;
                                            owl:someValuesFrom s4auto:Movement
                                          ] ,
                                          [ rdf:type owl:Restriction ;
                                            owl:onProperty s4auto:hasWidth ;
                                            owl:someValuesFrom s4auto:Width
                                          ] ;
                          rdfs:comment "Non-motorized road users as well as users of VRU vehicles (L class of vehicles, for example mopeds or motorcycles, etc.) participating to the road traffic" ;
                          rdfs:label "VulnerableRoadUser"@en .


###  https://saref.etsi.org/saref4auto/Weight
s4auto:Weight rdf:type owl:Class ;
              rdfs:subClassOf saref:Property ,
                              [ rdf:type owl:Restriction ;
                                owl:onProperty saref:hasValue ;
                                owl:someValuesFrom xsd:float
                              ] ;
              rdfs:comment "A Property of interest for the automotive domain"@en ;
              rdfs:label "Weight"@en .


###  https://saref.etsi.org/saref4auto/Width
s4auto:Width rdf:type owl:Class ;
             rdfs:subClassOf saref:Property ,
                             [ rdf:type owl:Restriction ;
                               owl:onProperty saref:hasValue ;
                               owl:someValuesFrom xsd:float
                             ] ;
             rdfs:comment "A Property of interest for the automotive domain"@en ;
             rdfs:label "Width"@en .


###  https://saref.etsi.org/saref4auto/WidthUnit
s4auto:WidthUnit rdf:type owl:Class ;
                 rdfs:subClassOf saref:UnitOfMeasure ;
                 rdfs:comment "unit of measure of width"@en ;
                 rdfs:label "width unit"@en .


###  https://saref.etsi.org/saref4auto/YawRate
s4auto:YawRate rdf:type owl:Class ;
               rdfs:subClassOf s4auto:Heading ;
               rdfs:comment "A type of heading"@en ;
               rdfs:label "YawRate"@en .


###  https://saref.etsi.org/saref4syst/System
s4syst:System rdf:type owl:Class ;
              rdfs:comment "The class of systems, i.e., systems virtually isolated from the environment, whose behaviour and interactions with the environment are modeled. Systems can be connected to other systems. Connected systems interact in some ways. Systems can also have subsystems. Properties of subsystems somehow contribute to the properties of the supersystem"@en ;
              rdfs:isDefinedBy s4syst: ;
              rdfs:label "System"@en .


#################################################################
#    Individuals
#################################################################

###  https://saref.etsi.org/saref4auto/Agriculture
s4auto:Agriculture rdf:type owl:NamedIndividual ,
                            s4auto:VehicleRole ;
                   rdfs:comment "A type of vehicle role"@en ;
                   rdfs:label "agriculture"@en .


###  https://saref.etsi.org/saref4auto/Commercial
s4auto:Commercial rdf:type owl:NamedIndividual ,
                           s4auto:VehicleRole ;
                  rdfs:comment "A type of vehicle role"@en ;
                  rdfs:label "commercial"@en .


###  https://saref.etsi.org/saref4auto/CrossingLeft
s4auto:CrossingLeft rdf:type owl:NamedIndividual ,
                             s4auto:Movement ;
                    rdfs:comment "A type of movement"@en ;
                    rdfs:label "crossing Left"@en .


###  https://saref.etsi.org/saref4auto/CrossingRight
s4auto:CrossingRight rdf:type owl:NamedIndividual ,
                              s4auto:Movement ;
                     rdfs:comment "A type of movement"@en ;
                     rdfs:label "crossing Right"@en .


###  https://saref.etsi.org/saref4auto/DangerousGood
s4auto:DangerousGood rdf:type owl:NamedIndividual ,
                              s4auto:VehicleRole ;
                     rdfs:comment "A type of vehicle role"@en ;
                     rdfs:label "dangerousGoods"@en .


###  https://saref.etsi.org/saref4auto/Emergency
s4auto:Emergency rdf:type owl:NamedIndividual ,
                          s4auto:VehicleRole ;
                 rdfs:comment "A type of vehicle role"@en ;
                 rdfs:label "emergency"@en .


###  https://saref.etsi.org/saref4auto/Follower
s4auto:Follower rdf:type owl:NamedIndividual ,
                         s4auto:PlatoonRole ;
                rdfs:comment "A type of platoon role"@en ;
                rdfs:label "follower"@en .


###  https://saref.etsi.org/saref4auto/Leader
s4auto:Leader rdf:type owl:NamedIndividual ,
                       s4auto:PlatoonRole ;
              rdfs:comment "A type of platoon role"@en ;
              rdfs:label "leader"@en .


###  https://saref.etsi.org/saref4auto/Military
s4auto:Military rdf:type owl:NamedIndividual ,
                         s4auto:VehicleRole ;
                rdfs:comment "A type of vehicle role"@en ;
                rdfs:label "military"@en .


###  https://saref.etsi.org/saref4auto/PublicTransport
s4auto:PublicTransport rdf:type owl:NamedIndividual ,
                                s4auto:VehicleRole .


###  https://saref.etsi.org/saref4auto/ReadyForLeading
s4auto:ReadyForLeading rdf:type owl:NamedIndividual ,
                                s4auto:PlatoonRole ;
                       rdfs:comment "A type of platoon role"@en ;
                       rdfs:label "ready for leading"@en .


###  https://saref.etsi.org/saref4auto/Rescue
s4auto:Rescue rdf:type owl:NamedIndividual ,
                       s4auto:VehicleRole ;
              rdfs:comment "A type of vehicle role"@en ;
              rdfs:label "rescue"@en .


###  https://saref.etsi.org/saref4auto/ReverseDirection
s4auto:ReverseDirection rdf:type owl:NamedIndividual ,
                                 s4auto:Movement ;
                        rdfs:comment "A type of movement"@en ;
                        rdfs:label "reverse Direction"@en .


###  https://saref.etsi.org/saref4auto/RoadOperator
s4auto:RoadOperator rdf:type owl:NamedIndividual ,
                             s4auto:VehicleRole ;
                    rdfs:comment "A type of vehicle role"@en ;
                    rdfs:label "roadOperator"@en .


###  https://saref.etsi.org/saref4auto/RoadWork
s4auto:RoadWork rdf:type owl:NamedIndividual ,
                         s4auto:VehicleRole ;
                rdfs:comment "A type of vehicle role"@en ;
                rdfs:label "roadWork"@en .


###  https://saref.etsi.org/saref4auto/SafetyCar
s4auto:SafetyCar rdf:type owl:NamedIndividual ,
                          s4auto:VehicleRole ;
                 rdfs:comment "A type of vehicle role"@en ;
                 rdfs:label "safetyCar"@en .


###  https://saref.etsi.org/saref4auto/SameDirection
s4auto:SameDirection rdf:type owl:NamedIndividual ,
                              s4auto:Movement ;
                     rdfs:comment "A type of movement"@en ;
                     rdfs:label "same Direction"@en .


###  https://saref.etsi.org/saref4auto/SpecialTransport
s4auto:SpecialTransport rdf:type owl:NamedIndividual ,
                                 s4auto:VehicleRole ;
                        rdfs:comment "A type of vehicle role"@en ;
                        rdfs:label "specialTransport"@en .


###  https://saref.etsi.org/saref4auto/Static
s4auto:Static rdf:type owl:NamedIndividual ,
                       s4auto:Movement ;
              rdfs:comment "A type of movement"@en ;
              rdfs:label "static"@en .


###  https://saref.etsi.org/saref4auto/Taxi
s4auto:Taxi rdf:type owl:NamedIndividual ,
                     s4auto:VehicleRole ;
            rdfs:comment "A type of vehicle role"@en ;
            rdfs:label "taxi"@en .


###  https://saref.etsi.org/saref4auto/Trailing
s4auto:Trailing rdf:type owl:NamedIndividual ,
                         s4auto:PlatoonRole ;
                rdfs:comment "A type of platoon role"@en ;
                rdfs:label "trailing"@en .


###  https://saref.etsi.org/saref4auto/Unknown
s4auto:Unknown rdf:type owl:NamedIndividual ,
                        s4auto:PlatoonRole .


#################################################################
#    Annotations
#################################################################

s4auto:PublicTransport rdfs:comment "A type of vehicle role"@en ;
                       rdfs:label "PublicTransport"@en ,
                                  "publicTransport"@en ;
                       rdfs:comment "A type of vehicle. Example of public transport is a bus or a tram"@en .


s4auto:Unknown rdfs:comment "A type of state for Platoon or for a Vehicle in a Platoon"@en ,
                            "A type of platoon role"@en ;
               rdfs:label "unknown"@en .


#################################################################
#    General axioms
#################################################################

[ rdf:type owl:AllDisjointClasses ;
  owl:members ( s4auto:OWLClass_083fab3f_ca95_4af8_873e_7563bd6bec77
                s4auto:OWLClass_7f65788c_8f5a_4c8b_89c8_1f924c8ef511
                s4auto:OWLClass_8ef04dbb_f94e_4dae_8bf0_cb63cd807909
                s4auto:OWLClass_f12ac0e6_d518_41b2_a737_112009debde8
              )
] .


[ rdf:type owl:AllDisjointClasses ;
  owl:members ( s4auto:OWLClass_268735bf_d97b_43a0_80f7_ead69c3861fa
                s4auto:OWLClass_c74dee04_0497_4156_bcad_06a79021d4b3
                s4auto:OWLClass_d2f64388_08b5_4626_8be5_bf2614562bb8
                s4auto:OWLClass_efb5f3dd_4e42_4e19_91b3_f451575038ea
              )
] .


[ rdf:type owl:AllDisjointClasses ;
  owl:members ( s4auto:OWLClass_3ef5abd6_4002_4095_96dd_008e5780e633
                s4auto:OWLClass_495b7639_fa49_44c2_a634_3838926ad786
                s4auto:OWLClass_62ab1c22_189c_4445_85ee_1ef1e2d17b57
                s4auto:OWLClass_8cd541c9_9bb2_49a5_9820_43c0dbcf5a60
                s4auto:OWLClass_c25f950f_505d_4814_be70_0de84bc70d3c
                s4auto:OWLClass_f4d3087f_4c57_4b40_bbf0_59a10d4f1876
              )
] .


[ rdf:type owl:AllDisjointClasses ;
  owl:members ( s4auto:OWLClass_92454d09_d714_4870_a8d4_c8c16bbc49d8
                s4auto:OWLClass_92dab589_1afc_4f99_a53c_031ddf5a1d85
                s4auto:OWLClass_eb1fda7a_fc6c_4dfb_ac2f_1ce59234bc97
              )
] .


###  Generated by the OWL API (version 4.5.9.2019-02-01T07:24:44Z) https://github.com/owlcs/owlapi
